field_at

floyd/field_at.v
@@ -11,7 +11,7 @@ Require Import VST.floyd.jmeq_lemmas.
 Require Import VST.zlist.sublist.
 Import LiftNotation.
 
-Local Open Scope logic.
+Local Unset SsrRewrite.
 
 (************************************************
 
@@ -21,7 +21,7 @@ Definition of nested_reptype_structlist, field_at, array_at, data_at, nested_sfi
 
 Section CENV.
 
-Context {cs: compspecs}.
+Context `{!heapGS Σ} {cs: compspecs}.
 
 Lemma struct_Prop_cons2:
   forall it it' m (A: member -> Type)
@@ -54,8 +54,7 @@ Proof.
     destruct (member_dec a0 a0); [ | congruence].
     unfold eq_rect_r in H0; rewrite <- !eq_rect_eq in H0.
     simpl. auto.
-  +
-    revert H1.
+  + revert H1.
     change (struct_Prop (a0 :: a1 :: m) P0 v0) with
       (P0 a0 (fst v0) /\ struct_Prop (a1 :: m) P0 (snd v0)).
     change (struct_Prop (a0 :: a1 :: m) P1 v1) with
@@ -74,7 +73,7 @@ Proof.
       unfold eq_rect_r; rewrite <- !eq_rect_eq.
       intros. apply (H0 (fst v0) (fst v1)); auto.
       hnf. left; reflexivity.
-    -  destruct H1 as [_ H1]; revert H1.
+    - destruct H1 as [_ H1]; revert H1.
       apply IHm; clear IHm.
       assert (name_member a0 <> name_member a1) by (contradict H; left; auto).
       intros.
@@ -122,7 +121,7 @@ Proof.
 Qed.
 
 Definition field_at (sh: Share.t) (t: type) (gfs: list gfield) (v: reptype (nested_field_type t gfs)) (p: val): mpred :=
- !! (field_compatible t gfs p) &&
+ ⌜field_compatible t gfs p⌝ ∧
  at_offset (data_at_rec sh (nested_field_type t gfs) v) (nested_field_offset t gfs) p.
 Arguments field_at sh t gfs v p : simpl never.
 
@@ -143,7 +142,7 @@ Definition nested_reptype_unionlist t gfs (m: members) :=
 
 Lemma map_members_ext: forall A (f f':member -> A) (m: list member),
   members_no_replicate m = true ->
-  (forall i, in_members i m -> f (get_member i m)= f' (get_member i m)) ->
+  (forall i, in_members i m -> f (get_member i m) = f' (get_member i m)) ->
   map f m = map f' m.
 Proof.
   intros.
@@ -196,7 +195,7 @@ Defined.
 
 Definition nested_sfieldlist_at sh t gfs m (v: nested_reptype_structlist t gfs m) p: mpred :=
   match m with
-  | nil => (!! field_compatible t gfs p) && emp
+  | nil => ⌜field_compatible t gfs p⌝ ∧ emp
   | _ => struct_pred m (fun it v p =>
            withspacer sh
             (nested_field_offset t gfs +
@@ -208,7 +207,7 @@ Definition nested_sfieldlist_at sh t gfs m (v: nested_reptype_structlist t gfs m
 
 Definition nested_ufieldlist_at sh t gfs m (v: nested_reptype_unionlist t gfs m) (p: val): mpred :=
   match m with
-  | nil => (!! field_compatible t gfs p) && emp
+  | nil => ⌜field_compatible t gfs p⌝ ∧ emp
   | _ => union_pred m (fun it v p =>
            withspacer sh
             (nested_field_offset t gfs + sizeof (field_type (name_member it) m))
@@ -218,8 +217,8 @@ Definition nested_ufieldlist_at sh t gfs m (v: nested_reptype_unionlist t gfs m)
 
 Definition array_at (sh: Share.t) (t: type) (gfs: list gfield) (lo hi: Z)
   (v: list (reptype (nested_field_type t (ArraySubsc 0 :: gfs)))) (p: val) : mpred :=
-  !! (field_compatible0 t (ArraySubsc lo :: gfs) p /\
-      field_compatible0 t (ArraySubsc hi :: gfs) p) &&
+  ⌜field_compatible0 t (ArraySubsc lo :: gfs) p /\
+   field_compatible0 t (ArraySubsc hi :: gfs) p⌝ ∧
   array_pred lo hi
     (fun i v => at_offset (data_at_rec sh (nested_field_type t (ArraySubsc 0 :: gfs)) v)
        (nested_field_offset t (ArraySubsc i :: gfs))) v p.
@@ -235,111 +234,106 @@ field_compatible, local_facts, isptr and offset_zero properties
 
 Lemma field_at_local_facts:
   forall sh t path v c,
-     field_at sh t path v c |-- !! (field_compatible t path c /\ value_fits (nested_field_type t path) v).
+     field_at sh t path v c ⊢ ⌜field_compatible t path c /\ value_fits (nested_field_type t path) v⌝.
 Proof.
   intros.
-  unfold field_at.
-  rewrite prop_and; apply andp_derives; auto.
-  unfold at_offset.
-  apply data_at_rec_value_fits.
+  unfold field_at, at_offset.
+  rewrite data_at_rec_value_fits.
+  by iIntros "(% & %)"; iPureIntro.
 Qed.
 
 Lemma field_at_compatible':
  forall sh t path v c,
-     field_at sh t path v c =
-     !! field_compatible t path c && field_at sh t path v c.
+     field_at sh t path v c ⊣⊢
+     ⌜field_compatible t path c⌝ ∧ field_at sh t path v c.
 Proof.
 intros.
-apply pred_ext.
-apply andp_right; auto.
-eapply derives_trans; [apply field_at_local_facts | normalize].
+iSplit; last by iIntros "(_ & $)".
+rewrite bi.and_comm; iApply add_and.
+rewrite field_at_local_facts.
 normalize.
 Qed.
 
 Lemma field_at__local_facts: forall sh t gfs p,
-  field_at_ sh t gfs p |-- !! field_compatible t gfs p.
+  field_at_ sh t gfs p ⊢ ⌜field_compatible t gfs p⌝.
 Proof.
   intros.
   unfold field_at_, field_at.
- normalize.
+  normalize.
 Qed.
 
 Lemma data_at_local_facts:
-   forall sh t v p, data_at sh t v p |-- !! (field_compatible t nil p /\ value_fits t v).
+   forall sh t v p, data_at sh t v p ⊢ ⌜field_compatible t nil p /\ value_fits t v⌝.
 Proof. intros. apply field_at_local_facts. Qed.
 
-Lemma data_at__local_facts: forall sh t p, data_at_ sh t p |-- !! field_compatible t nil p.
+Lemma data_at__local_facts: forall sh t p, data_at_ sh t p ⊢ ⌜field_compatible t nil p⌝.
 Proof. intros.
   apply field_at__local_facts.
 Qed.
 
 Lemma array_at_local_facts: forall sh t gfs lo hi v p,
-  array_at sh t gfs lo hi v p |--
-    !! (field_compatible0 t (ArraySubsc lo :: gfs) p
+  array_at sh t gfs lo hi v p ⊢
+    ⌜field_compatible0 t (ArraySubsc lo :: gfs) p
         /\ field_compatible0 t (ArraySubsc hi :: gfs) p
         /\ Zlength v = hi - lo
-        /\ Forall (value_fits (nested_field_type t (ArraySubsc 0 :: gfs))) v).
+        /\ Forall (value_fits (nested_field_type t (ArraySubsc 0 :: gfs))) v⌝.
 Proof.
   intros.
   unfold array_at.
-  rewrite !prop_and.
-  rewrite <- andp_assoc.
-  apply andp_derives; auto.
-  eapply derives_trans; [apply array_pred_local_facts |].
-  + intros.
-    unfold at_offset.
-    instantiate (1 := fun x => value_fits _ x).
-    apply data_at_rec_value_fits.
- + normalize.
+  rewrite array_pred_local_facts.
+  2: { intros.
+       unfold at_offset.
+       apply data_at_rec_value_fits. }
+  normalize.
 Qed.
 
 Lemma array_at__local_facts: forall sh t gfs lo hi p,
-  array_at_ sh t gfs lo hi p |--
-    !! (field_compatible0 t (ArraySubsc lo :: gfs) p
-        /\ field_compatible0 t (ArraySubsc hi :: gfs) p).
+  array_at_ sh t gfs lo hi p ⊢
+    ⌜field_compatible0 t (ArraySubsc lo :: gfs) p
+        /\ field_compatible0 t (ArraySubsc hi :: gfs) p⌝.
 Proof.
   intros.
   unfold array_at_.
-  eapply derives_trans; [apply array_at_local_facts; eauto | ].
-  apply prop_derives; intuition.
+  rewrite array_at_local_facts; eauto.
+  apply bi.pure_mono; intuition.
 Qed.
 
 Lemma field_at_isptr: forall sh t gfs v p,
-  field_at sh t gfs v p = (!! isptr p) && field_at sh t gfs v p.
+  field_at sh t gfs v p ⊣⊢ ⌜isptr p⌝ ∧ field_at sh t gfs v p.
 Proof. intros. eapply local_facts_isptr; [apply field_at_local_facts | intros [? ?]; auto]. Qed.
 
 Lemma field_at_offset_zero: forall sh t gfs v p,
-  field_at sh t gfs v p = field_at sh t gfs v (offset_val 0 p).
+  field_at sh t gfs v p ⊣⊢ field_at sh t gfs v (offset_val 0 p).
 Proof. intros. apply local_facts_offset_zero.
  intros. rewrite field_at_isptr; normalize.
 Qed.
 
 Lemma field_at__isptr: forall sh t gfs p,
-  field_at_ sh t gfs p = (!! isptr p) && field_at_ sh t gfs p.
+  field_at_ sh t gfs p ⊣⊢ ⌜isptr p⌝ ∧ field_at_ sh t gfs p.
 Proof. intros.
  intros. eapply local_facts_isptr; [apply field_at__local_facts | intros [? ?]; auto].
 Qed.
 
 Lemma field_at__offset_zero: forall sh t gfs p,
-  field_at_ sh t gfs p = field_at_ sh t gfs (offset_val 0 p).
+  field_at_ sh t gfs p ⊣⊢ field_at_ sh t gfs (offset_val 0 p).
 Proof. intros. apply local_facts_offset_zero.
  intros. rewrite field_at__isptr; normalize.
 Qed.
 
-Lemma data_at_isptr: forall sh t v p, data_at sh t v p = !!(isptr p) && data_at sh t v p.
+Lemma data_at_isptr: forall sh t v p, data_at sh t v p ⊣⊢ ⌜isptr p⌝ ∧ data_at sh t v p.
 Proof. intros. eapply local_facts_isptr; [apply data_at_local_facts | intros [? ?]; auto].
 Qed.
 
-Lemma data_at_offset_zero: forall sh t v p, data_at sh t v p = data_at sh t v (offset_val 0 p).
+Lemma data_at_offset_zero: forall sh t v p, data_at sh t v p ⊣⊢ data_at sh t v (offset_val 0 p).
 Proof. intros. rewrite <- local_facts_offset_zero. reflexivity.
     intros; rewrite data_at_isptr; normalize.
 Qed.
 
-Lemma data_at__isptr: forall sh t p, data_at_ sh t p = !!(isptr p) && data_at_ sh t p.
+Lemma data_at__isptr: forall sh t p, data_at_ sh t p ⊣⊢ ⌜isptr p⌝ ∧ data_at_ sh t p.
 Proof. intros. eapply local_facts_isptr; [apply data_at__local_facts | intros [? ?]; auto].
 Qed.
 
-Lemma data_at__offset_zero: forall sh t p, data_at_ sh t p = data_at_ sh t (offset_val 0 p).
+Lemma data_at__offset_zero: forall sh t p, data_at_ sh t p ⊣⊢ data_at_ sh t (offset_val 0 p).
 Proof. intros. apply field_at__offset_zero. Qed.
 
 (************************************************
@@ -354,9 +348,9 @@ Lemma array_at_ext_derives: forall sh t gfs lo hi v0 v1 p,
      lo <= i < hi ->
      JMeq u0 (Znth (i-lo) v0) ->
      JMeq u1 (Znth (i-lo) v1) ->
-     field_at sh t (ArraySubsc i :: gfs) u0 p |--
+     field_at sh t (ArraySubsc i :: gfs) u0 p ⊢
      field_at sh t (ArraySubsc i :: gfs) u1 p) ->
-  array_at sh t gfs lo hi v0 p |-- array_at sh t gfs lo hi v1 p.
+  array_at sh t gfs lo hi v0 p ⊢ array_at sh t gfs lo hi v1 p.
 Proof.
   intros until p. intro ZL; intros.
   unfold array_at, field_at.
@@ -382,14 +376,12 @@ Lemma array_at_ext: forall sh t gfs lo hi v0 v1 p,
      lo <= i < hi ->
      JMeq u0 (Znth (i-lo) v0) ->
      JMeq u1 (Znth (i-lo) v1) ->
-     field_at sh t (ArraySubsc i :: gfs) u0 p =
+     field_at sh t (ArraySubsc i :: gfs) u0 p ⊣⊢
      field_at sh t (ArraySubsc i :: gfs) u1 p) ->
-  array_at sh t gfs lo hi v0 p = array_at sh t gfs lo hi v1 p.
+  array_at sh t gfs lo hi v0 p ⊣⊢ array_at sh t gfs lo hi v1 p.
 Proof.
   intros.
-  apply pred_ext; apply array_at_ext_derives; intros; auto.
-  erewrite H0 by eauto; auto.
-  erewrite <- H0 by eauto; auto.
+  iSplit; iApply array_at_ext_derives; try done; intros; [rewrite H0 | rewrite <- H0]; done.
 Qed.
 
 (************************************************
@@ -403,7 +395,7 @@ Lemma field_at_Tarray: forall sh t gfs t0 n a v1 v2 p,
   nested_field_type t gfs = Tarray t0 n a ->
   0 <= n ->
   JMeq v1 v2 ->
-  field_at sh t gfs v1 p = array_at sh t gfs 0 n v2 p.
+  field_at sh t gfs v1 p ⊣⊢ array_at sh t gfs 0 n v2 p.
 Proof.
   intros.
   unfold field_at, array_at.
@@ -413,8 +405,8 @@ Proof.
   intros.
   rewrite data_at_rec_eq.
   rewrite at_offset_array_pred.
-  f_equal.
-  + apply ND_prop_ext.
+  apply bi.and_proper.
+  + f_equiv.
     rewrite !field_compatible0_cons, H0.
     assert (0 <= 0 <= n) by lia.
     assert (0 <= n <= n) by lia.
@@ -434,21 +426,18 @@ Proof.
       rewrite (nested_field_offset_ind t (ArraySubsc i :: gfs))
         by (apply legal_nested_field0_field; simpl; unfold legal_field; rewrite H0; auto).
       rewrite H0.
-      f_equal.
       subst; auto.
 Qed.
 
-Lemma not_ptr_FF: forall A p, (A |-- !! isptr p) <-> (~ isptr p -> A = FF).
+Lemma not_ptr_False: forall (A : mpred) p, (A ⊢ ⌜isptr p⌝) <-> (~ isptr p -> A ⊣⊢ False).
 Proof.
   intros.
   split; intros.
-  + apply pred_ext; [| apply FF_left].
-    eapply derives_trans; [eauto |].
-    apply prop_derives.
-    auto.
-  + destruct p; try solve [rewrite H by (simpl; congruence); apply FF_left].
-    simpl.
-    apply TT_right.
+  + iSplit; last by iIntros "[]".
+    rewrite H; iIntros (?); done.
+  + destruct (isptr_dec p); first by iIntros "_".
+    rewrite H; last done.
+    iIntros "[]".
 Qed.
 
 Ltac solve_ptr_derives :=
@@ -456,40 +445,40 @@ Ltac solve_ptr_derives :=
   apply derives_refl.
 
 Lemma field_at_isptr':
-  forall sh t path v c, field_at sh t path v c |-- !! isptr c.
+  forall sh t path v c, field_at sh t path v c ⊢ ⌜isptr c⌝.
 Proof.
 intros.
-eapply derives_trans; [apply field_at_local_facts | ].
-apply prop_derives; intros [? _]; auto.
+rewrite field_at_local_facts.
+iIntros "(($ & _) & _)".
 Qed.
 
 Ltac solve_nptr p A :=
   let H := fresh "H" in
   match A with
-  | (?B * ?C) % logic =>
-     try solve [assert (~ isptr p -> B = FF) as H by solve_nptr p B;
-                intro; rewrite H by auto ; apply FF_sepcon];
-     try solve [assert (~ isptr p -> C = FF) as H by solve_nptr p C;
-                intro; rewrite H by auto; apply sepcon_FF]
-  | (?B && ?C) % logic =>
-     try solve [assert (~ isptr p -> B = FF) as H by solve_nptr p B;
-                intro; rewrite H by auto ; apply FF_andp];
-     try solve [assert (~ isptr p -> C = FF) as H by solve_nptr p C;
-                intro; rewrite H by auto; apply andp_FF]
-  | _ => apply (proj1 (not_ptr_FF A p)); solve_ptr p A
+  | (?B ∗ ?C) =>
+     try solve [assert (~ isptr p -> B ⊣⊢ False) as H by solve_nptr p B;
+                intro; rewrite H by auto; apply bi.False_sep];
+     try solve [assert (~ isptr p -> C ⊣⊢ False) as H by solve_nptr p C;
+                intro; rewrite H by auto; apply bi.sep_False]
+  | (?B ∧ ?C) =>
+     try solve [assert (~ isptr p -> B ⊣⊢ False) as H by solve_nptr p B;
+                intro; rewrite H by auto; apply bi.False_and];
+     try solve [assert (~ isptr p -> C ⊣⊢ False) as H by solve_nptr p C;
+                intro; rewrite H by auto; apply bi.and_False]
+  | _ => apply (proj1 (not_ptr_False A p)); solve_ptr p A
   end
 with solve_ptr p A :=
   let p0 := fresh "p" in
   match A with
-  | (_ * _) % logic => apply (proj2 (not_ptr_FF A p)); solve_nptr p A
-  | (_ && _) % logic => apply (proj2 (not_ptr_FF A p)); solve_nptr p A
-  | (!! _ /\ _)%logic => destruct A as [_ A]; solve_ptr p A
-  | (!! field_compatible _ _ ?q) => apply (derives_trans _ _ _ (prop_derives _ _ (field_compatible_isptr _ _ _))); solve_ptr_derives
-  | (!! field_compatible0 _ _ ?q) => apply (derives_trans _ _ _ (prop_derives _ _ (field_compatible0_isptr _ _ _))); solve_ptr_derives
-  | (memory_block _ _ ?q) => apply (derives_trans _ _ _ (memory_block_local_facts _ _ _)); solve_ptr_derives
+  | (_ ∗ _) => apply (proj2 (not_ptr_False A p)); solve_nptr p A
+  | (_ ∧ _) => apply (proj2 (not_ptr_False A p)); solve_nptr p A
+  | ⌜_ /\ _⌝ => destruct A as [_ A]; solve_ptr p A
+  | ⌜field_compatible _ _ ?q⌝ => etrans; first apply (bi.pure_mono _ _ (field_compatible_isptr _ _ _)); solve_ptr_derives
+  | ⌜field_compatible0 _ _ ?q⌝ => etrans; first apply (bi.pure_mono _ _ (field_compatible0_isptr _ _ _)); solve_ptr_derives
+  | (memory_block _ _ ?q) => etrans; first apply (memory_block_local_facts _ _ _); solve_ptr_derives
   | (withspacer _ _ _ ?P p) => apply withspacer_preserve_local_facts;
                                      intro p0; solve_ptr p0 (P p0)
-  | (at_offset ?P _ ?q) => apply (derives_trans _ (!! isptr q));
+  | (at_offset ?P _ ?q) => trans ⌜isptr q⌝;
                            [apply at_offset_preserve_local_facts; intro p0; solve_ptr p0 (P p0) |
                             solve_ptr_derives]
   | (field_at _ _ _ _ p) => apply field_at_isptr'
@@ -499,18 +488,18 @@ Ltac destruct_ptr p :=
   let b := fresh "b" in
   let ofs := fresh "OFS" in
   match goal with
-  | |- (@eq mpred) ?A ?B =>
+  | |- ?A ⊣⊢ ?B =>
        let H := fresh "H" in
        let H0 := fresh "H" in
-       assert (~ isptr p -> A = FF) as H by solve_nptr p A;
-       assert (~ isptr p -> B = FF) as H0 by solve_nptr p B;
+       assert (~ isptr p -> A ⊣⊢ False) as H by solve_nptr p A;
+       assert (~ isptr p -> B ⊣⊢ False) as H0 by solve_nptr p B;
        destruct p as [| | | | | b ofs]; try (rewrite H, H0 by (simpl; congruence); reflexivity);
        clear H H0;
        inv_int ofs
-  | |- (?A |-- _) =>
+  | |- (?A ⊢ _) =>
        let H := fresh "H" in
-       assert (~ isptr p -> A = FF) as H by solve_nptr p A;
-       destruct p as [| | | | | b ofs]; try (rewrite H by (simpl; congruence); apply FF_left);
+       assert (~ isptr p -> A ⊣⊢ False) as H by solve_nptr p A;
+       destruct p as [| | | | | b ofs]; try (rewrite H by (simpl; congruence); apply bi.False_elim);
        clear H;
        inv_int ofs
   end.
@@ -518,14 +507,14 @@ Ltac destruct_ptr p :=
 Lemma field_at_Tstruct: forall sh t gfs id a v1 v2 p,
   nested_field_type t gfs = Tstruct id a ->
   JMeq v1 v2 ->
-  field_at sh t gfs v1 p = nested_sfieldlist_at sh t gfs (co_members (get_co id)) v2 p.
+  field_at sh t gfs v1 p ⊣⊢ nested_sfieldlist_at sh t gfs (co_members (get_co id)) v2 p.
 Proof.
   intros.
   unfold field_at, nested_sfieldlist_at.
   revert v1 H0; rewrite H; intros.
   rewrite data_at_rec_eq.
   rewrite at_offset_struct_pred.
-  rewrite andp_struct_pred by apply corable_prop.
+  rewrite andp_struct_pred; [| apply _..].
   generalize (co_members (get_co id)) at 1 10; intro m; destruct m; [auto |].
   apply struct_pred_ext; [apply get_co_members_no_replicate |].
 
@@ -546,14 +535,14 @@ Proof.
     by (clear - n H H1; unfold field_compatible; simpl in *; rewrite H in *; simpl in *; tauto).
     rewrite !prop_false_andp by auto; auto.
   }
-  f_equal.
+  f_equiv.
   {
-   f_equal.
+   f_equiv.
    unfold field_compatible.
-   f_equal. f_equal. f_equal. f_equal.
-   simpl. apply prop_ext.
+   do 4 f_equiv.
+   simpl.
    split; intro; try tauto. split; auto.
-    rewrite H. simpl. rewrite name_member_get. auto.
+   rewrite H. simpl. rewrite name_member_get. auto.
   }
   replace  (field_offset cenv_cs (name_member (get_member i (co_members (get_co id)))))
    with  (field_offset cenv_cs i)
@@ -561,24 +550,23 @@ Proof.
   replace  (field_offset_next cenv_cs (name_member (get_member i (co_members (get_co id)))))
    with  (field_offset_next cenv_cs i)
     by (rewrite name_member_get; auto).
-  f_equal.
-  f_equal.
+  apply bi.sep_proper.
+  f_equiv.
   rewrite name_member_get.
   change (sizeof ?A) with (expr.sizeof A) in *.
-  rewrite sizeof_Tstruct. lia.
-  f_equal. f_equal.
+  rewrite sizeof_Tstruct. hnf; lia.
+  hnf; f_equal. f_equal.
   rewrite name_member_get.  lia.
-  match goal with |- data_at_rec _ _ _ ?A = data_at_rec _ _ _ ?B => replace B with A end.
- 2:{ f_equal. f_equal.
+  match goal with |- data_at_rec _ _ _ ?A ⊣⊢ data_at_rec _ _ _ ?B => replace B with A end.
+  2:{ f_equal. f_equal.
   rewrite name_member_get.
   rewrite @nested_field_offset_ind with (gfs := StructField i :: gfs) by auto.
   unfold gfield_offset; rewrite H. lia.
   }
-  apply equal_f.
-  apply data_at_rec_type_changable.
-  rewrite nested_field_type_ind.
-      simpl; rewrite H.
-      auto.
+  erewrite data_at_rec_type_changable; first done.
+  { rewrite nested_field_type_ind.
+    simpl; rewrite H.
+    auto. }
   apply (proj_compact_prod_JMeq _ (get_member i _) (co_members (get_co id)) _ _ (unfold_reptype v1) v2); auto.
       * intros.
         rewrite nested_field_type_ind, H.
@@ -593,14 +581,14 @@ Qed.
 Lemma field_at_Tunion: forall sh t gfs id a v1 v2 p,
   nested_field_type t gfs = Tunion id a ->
   JMeq v1 v2 ->
-  field_at sh t gfs v1 p = nested_ufieldlist_at sh t gfs (co_members (get_co id)) v2 p.
+  field_at sh t gfs v1 p ⊣⊢ nested_ufieldlist_at sh t gfs (co_members (get_co id)) v2 p.
 Proof.
   intros.
   unfold field_at, nested_ufieldlist_at.
   revert v1 H0; rewrite H; intros.
   rewrite data_at_rec_eq.
   rewrite at_offset_union_pred.
-  rewrite andp_union_pred by apply corable_prop.
+  rewrite andp_union_pred; [| apply _..].
   generalize (eq_refl (co_members (get_co id))).
   generalize (co_members (get_co id)) at 2 3 9; intro m; destruct m; [auto |].
   intro HH; assert (co_members (get_co id) <> nil) by congruence; clear HH.
@@ -621,29 +609,28 @@ Proof.
   normalize.
   destruct (legal_nested_field_dec t (UnionField i :: gfs)).
   2:{
-    replace (!!field_compatible t (UnionField (name_member (get_member i (co_members (get_co id)))) :: gfs) (Vptr b (Ptrofs.repr ofs)) : mpred) with (FF: mpred)
-     by (rewrite name_member_get; apply ND_prop_ext; unfold field_compatible; tauto).
+    rewrite (bi.pure_False (field_compatible t (UnionField _ :: _) _))
+      by (rewrite name_member_get; unfold field_compatible; tauto).
     simpl in n.
     rewrite H in n.
     simpl in n.
-    replace (!!field_compatible t gfs (Vptr b (Ptrofs.repr ofs)) : mpred) with (FF: mpred)
-      by (apply ND_prop_ext; unfold field_compatible; tauto).
-    normalize.
+    rewrite bi.pure_False by (unfold field_compatible; tauto).
+    iSplit; iIntros "([] & ?)".
   }
-  f_equal.
-  apply ND_prop_ext.
+  f_equiv.
+  apply bi.pure_iff.
   rewrite name_member_get, field_compatible_cons, H; tauto.
-  f_equal. rewrite name_member_get.
-  f_equal. rewrite sizeof_Tunion. lia.
-  f_equal. f_equal. lia.
-  match goal with |- data_at_rec _ _ _ ?A = data_at_rec _ _ _ ?B => replace B with A end.
- 2:{ f_equal. f_equal.
+  apply bi.sep_proper.
+  rewrite name_member_get.
+  f_equiv. rewrite sizeof_Tunion. hnf; lia.
+  hnf; f_equal. f_equal. lia.
+  match goal with |- data_at_rec _ _ _ ?A ⊣⊢ data_at_rec _ _ _ ?B => replace B with A end.
+  2:{ f_equal. f_equal.
   rewrite name_member_get.
   rewrite @nested_field_offset_ind with (gfs := UnionField i :: gfs) by auto.
   unfold gfield_offset; rewrite H. lia.
   }
-  apply equal_f.
-  apply data_at_rec_type_changable.
+  erewrite data_at_rec_type_changable; first done.
   rewrite name_member_get.
   rewrite nested_field_type_ind.
   rewrite H; reflexivity.
@@ -657,17 +644,17 @@ Proof.
 Qed.
 
 Lemma array_at_len_0: forall sh t gfs i p,
-  array_at sh t gfs i i nil p = !! (field_compatible0 t (ArraySubsc i :: gfs) p) && emp.
+  array_at sh t gfs i i nil p ⊣⊢ ⌜field_compatible0 t (ArraySubsc i :: gfs) p⌝ ∧ emp.
 Proof.
   intros.
   unfold array_at.
   rewrite array_pred_len_0 by lia.
-  apply pred_ext; normalize.
+  apply bi.equiv_entails_2; normalize.
 Qed.
 
 Lemma array_at_len_1: forall sh t gfs i v v' p,
   JMeq v v' ->
-  array_at sh t gfs i (i + 1) (v :: nil) p = field_at sh t (ArraySubsc i :: gfs) v' p.
+  array_at sh t gfs i (i + 1) (v :: nil) p ⊣⊢ field_at sh t (ArraySubsc i :: gfs) v' p.
 Proof.
   intros.
   unfold array_at, field_at.
@@ -676,8 +663,8 @@ Proof.
   rewrite @nested_field_type_ArraySubsc with (i := i).
   intros.
   apply JMeq_eq in H; rewrite H.
-  f_equal.
-  apply ND_prop_ext.
+  apply bi.and_proper; last done.
+  apply bi.pure_iff.
   rewrite field_compatible_field_compatible0'.
   reflexivity.
 Qed.
@@ -685,8 +672,8 @@ Qed.
 Lemma split2_array_at: forall sh t gfs lo mid hi v p,
   lo <= mid <= hi ->
   Zlength v = hi - lo ->
-  array_at sh t gfs lo hi v p =
-  array_at sh t gfs lo mid (sublist 0 (mid-lo) v) p *
+  array_at sh t gfs lo hi v p ⊣⊢
+  array_at sh t gfs lo mid (sublist 0 (mid-lo) v) p ∗
   array_at sh t gfs mid hi (sublist (mid-lo) (Zlength v) v) p.
 Proof.
   intros.
@@ -707,14 +694,14 @@ Lemma split3seg_array_at: forall sh t gfs lo ml mr hi v p,
   ml <= mr ->
   mr <= hi ->
   Zlength v = hi-lo ->
-  array_at sh t gfs lo hi v p =
-    array_at sh t gfs lo ml (sublist 0 (ml-lo) v) p*
-    array_at sh t gfs ml mr (sublist (ml-lo) (mr-lo) v) p *
+  array_at sh t gfs lo hi v p ⊣⊢
+    array_at sh t gfs lo ml (sublist 0 (ml-lo) v) p ∗
+    array_at sh t gfs ml mr (sublist (ml-lo) (mr-lo) v) p ∗
     array_at sh t gfs mr hi (sublist (mr-lo) (hi-lo) v) p.
 Proof.
   intros.
   rewrite split2_array_at with (lo := lo) (mid := ml) (hi := hi) by lia.
-  rewrite sepcon_assoc; f_equal.
+  apply bi.sep_proper; first done.
   assert (Zlength (sublist (ml - lo) (hi - lo) v) = hi - ml).
   {
     replace (hi - ml) with (hi - lo - (ml - lo)) by lia.
@@ -722,26 +709,26 @@ Proof.
   }
   rewrite H2.
   rewrite split2_array_at with (lo := ml) (mid := mr) (hi := hi) by lia.
-  f_equal.
-  rewrite sublist_sublist; try lia. f_equal.  f_equal; lia.
+  apply bi.sep_proper.
+  rewrite sublist_sublist; try lia. f_equiv. f_equal; lia.
   rewrite Zlength_sublist by lia.
-  rewrite sublist_sublist; try lia. f_equal.  f_equal; lia.
+  rewrite sublist_sublist; try lia. f_equiv. f_equal; lia.
 Qed.
 
 Lemma split3_array_at: forall sh t gfs lo mid hi v v0 p,
   lo <= mid < hi ->
   Zlength v = hi-lo ->
   JMeq v0 (Znth (mid-lo) v) ->
-  array_at sh t gfs lo hi v p =
-    array_at sh t gfs lo mid (sublist 0 (mid-lo) v) p *
-    field_at sh t (ArraySubsc mid :: gfs) v0 p *
+  array_at sh t gfs lo hi v p ⊣⊢
+    array_at sh t gfs lo mid (sublist 0 (mid-lo) v) p ∗
+    field_at sh t (ArraySubsc mid :: gfs) v0 p ∗
     array_at sh t gfs (mid + 1) hi (sublist (mid+1-lo) (hi-lo) v) p.
 Proof.
   intros.
   rename H0 into e; rename H1 into H0.
   rewrite split3seg_array_at with (ml := mid) (mr := mid + 1) by lia.
-  f_equal.
-  f_equal.
+  apply bi.sep_proper; first done.
+  apply bi.sep_proper; last done.
   replace (mid + 1 - lo) with (mid - lo + 1) by lia.
   rewrite sublist_len_1 by lia.
   rewrite array_at_len_1 with (v' :=v0); [auto |].
@@ -755,7 +742,7 @@ Reroot lemmas
 ************************************************)
 
 Lemma field_at_data_at: forall sh t gfs v (p: val),
-  field_at sh t gfs v p =
+  field_at sh t gfs v p ⊣⊢
   data_at sh (nested_field_type t gfs) v (field_address t gfs p).
 Proof.
   intros.
@@ -768,11 +755,11 @@ Proof.
     destruct p; try (destruct H; contradiction).
     generalize (field_compatible_nested_field t gfs (Vptr b i));
     unfold at_offset; solve_mod_modulus; intros. auto.
-  + apply pred_ext; normalize. destruct H0; contradiction.
+  + apply bi.equiv_entails_2; normalize. destruct H0; contradiction.
 Qed.
 
-Lemma field_at_data_at' : forall sh t gfs v p, field_at sh t gfs v p =
-  !!field_compatible t gfs p &&
+Lemma field_at_data_at' : forall sh t gfs v p, field_at sh t gfs v p ⊣⊢
+  ⌜field_compatible t gfs p⌝ ∧
   data_at sh (nested_field_type t gfs) v (offset_val (nested_field_offset t gfs) p).
 Proof.
   intros.
@@ -785,7 +772,7 @@ Proof.
 Qed.
 
 Lemma field_at__data_at_: forall sh t gfs p,
-  field_at_ sh t gfs p =
+  field_at_ sh t gfs p ⊣⊢
   data_at_ sh (nested_field_type t gfs) (field_address t gfs p).
 Proof.
   intros.
@@ -793,22 +780,20 @@ Proof.
 Qed.
 
 Lemma lifted_field_at_data_at: forall sh t gfs v p,
-  `(field_at sh t gfs) v p =
-  `(data_at sh (nested_field_type t gfs)) v (`(field_address t gfs) p).
+  assert_of (`(field_at sh t gfs) v p) ⊣⊢
+  assert_of (`(data_at sh (nested_field_type t gfs)) v (`(field_address t gfs) p)).
 Proof.
   intros.
-  extensionality rho.
-  unfold liftx, lift; simpl.
+  split => rho; unfold_lift; simpl.
   apply field_at_data_at.
 Qed.
 
 Lemma lifted_field_at__data_at_: forall sh t gfs p,
-  `(field_at_ sh t gfs) p =
-  `(data_at_ sh (nested_field_type t gfs)) (`(field_address t gfs) p).
+  assert_of (`(field_at_ sh t gfs) p) ⊣⊢
+  assert_of (`(data_at_ sh (nested_field_type t gfs)) (`(field_address t gfs) p)).
 Proof.
   intros.
-  extensionality rho.
-  unfold liftx, lift; simpl.
+  split => rho; unfold_lift; simpl.
   apply field_at__data_at_.
 Qed.
 
@@ -822,9 +807,9 @@ Qed.
 
 Lemma array_at_data_at: forall sh t gfs lo hi v p,
   lo <= hi ->
-  array_at sh t gfs lo hi v p =
-  (!! field_compatible0 t (ArraySubsc lo :: gfs) p) &&
-  (!! field_compatible0 t (ArraySubsc hi :: gfs) p) &&
+  array_at sh t gfs lo hi v p ⊣⊢
+  ⌜field_compatible0 t (ArraySubsc lo :: gfs) p⌝ ∧
+  ⌜field_compatible0 t (ArraySubsc hi :: gfs) p⌝ ∧
   at_offset (data_at sh (nested_field_array_type t gfs lo hi) v)
                (nested_field_offset t (ArraySubsc lo :: gfs)) p.
 Proof.
@@ -839,7 +824,6 @@ Proof.
   rewrite <- at_offset_eq.
   normalize.
   apply andp_prop_ext.
-  f_equal.
   + pose proof field_compatible0_nested_field_array t gfs lo hi p.
     tauto.
   + intros [? ?].
@@ -850,8 +834,7 @@ Proof.
     intros.
     rewrite at_offset_eq at 1.
     rewrite at_offset_eq, <- at_offset_eq2, at_offset_eq.
-    f_equal.
-    f_equal.
+    f_equiv.
     f_equal.
     rewrite @nested_field_offset_ind with (gfs := nil) by (apply (field_compatible0_nested_field_array t gfs lo hi p); auto).
     assert (field_compatible0 t (gfs SUB i') p)
@@ -871,7 +854,7 @@ forall sh t gfs lo hi v p,
   lo <= hi ->
   field_compatible0 t (ArraySubsc lo :: gfs) p ->
   field_compatible0 t (ArraySubsc hi :: gfs) p ->
-  array_at sh t gfs lo hi v p =
+  array_at sh t gfs lo hi v p ⊣⊢
   data_at sh (nested_field_array_type t gfs lo hi) v
                (field_address0 t (ArraySubsc lo::gfs) p).
 Proof.
@@ -879,7 +862,7 @@ Proof.
   rewrite array_at_data_at by auto.
   rewrite !prop_true_andp by auto.
   unfold at_offset.
-  f_equal.
+  f_equiv.
   unfold field_address0.
   rewrite if_true; auto.
 Qed.
@@ -888,7 +871,7 @@ Lemma array_at_data_at'':
 forall sh t gfs lo hi v p,
   lo <= hi ->
   field_compatible0 t (ArraySubsc hi :: gfs) p ->
-  array_at sh t gfs lo hi v p =
+  array_at sh t gfs lo hi v p ⊣⊢
   data_at sh (nested_field_array_type t gfs lo hi) v
                (field_address0 t (ArraySubsc lo::gfs) p).
 Proof.
@@ -899,7 +882,7 @@ Proof.
   if_tac.
   + rewrite !prop_true_andp by auto.
     auto.
-  + apply pred_ext.
+  + apply bi.equiv_entails_2.
     - normalize.
     - rewrite data_at_isptr.
       normalize.
@@ -909,7 +892,7 @@ Lemma array_at_data_at''':
   forall sh t gfs lo hi v p t0 n a,
   nested_field_type t gfs = Tarray t0 n a ->
   lo <= hi <= n ->
-  array_at sh t gfs lo hi v p =
+  array_at sh t gfs lo hi v p ⊣⊢
   data_at sh (nested_field_array_type t gfs lo hi) v
                (field_address0 t (ArraySubsc lo::gfs) p).
 Proof.
@@ -927,7 +910,7 @@ Proof.
       lia.
     - rewrite !prop_true_andp by auto.
       auto.
-  + apply pred_ext.
+  + apply bi.equiv_entails_2.
     - normalize.
     - rewrite data_at_isptr.
       normalize.
@@ -938,11 +921,11 @@ Lemma split3seg_array_at': forall sh t gfs lo ml mr hi v p,
   ml <= mr ->
   mr <= hi ->
   Zlength v = hi-lo ->
-  array_at sh t gfs lo hi v p =
-    array_at sh t gfs lo ml (sublist 0 (ml-lo) v) p*
+  array_at sh t gfs lo hi v p ⊣⊢
+    array_at sh t gfs lo ml (sublist 0 (ml-lo) v) p ∗
     data_at sh (nested_field_array_type t gfs ml mr)
         (sublist (ml-lo) (mr-lo) v)
-               (field_address0 t (ArraySubsc ml::gfs) p) *
+               (field_address0 t (ArraySubsc ml::gfs) p) ∗
     array_at sh t gfs mr hi (sublist (mr-lo) (hi-lo) v) p.
 Proof.
   intros.
@@ -961,13 +944,13 @@ Lemmas about underscore and memory_block
 ************************************************)
 
 Lemma field_at_field_at_: forall sh t gfs v p,
-  field_at sh t gfs v p |-- field_at_ sh t gfs p.
+  field_at sh t gfs v p ⊢ field_at_ sh t gfs p.
 Proof.
   intros.
   destruct (field_compatible_dec t gfs p).
   + destruct_ptr p.
     unfold field_at_, field_at.
-    apply andp_derives; auto.
+    apply bi.and_mono; first done.
     pose proof field_compatible_nested_field _ _ _ f.
     unfold field_compatible in H, f.
     unfold offset_val in H.
@@ -990,14 +973,14 @@ Qed.
 
 Lemma field_at_field_at_default : forall sh t gfs v v' p,
   v' = default_val (nested_field_type t gfs) ->
-  field_at sh t gfs v p |-- field_at sh t gfs v' p.
+  field_at sh t gfs v p ⊢ field_at sh t gfs v' p.
 Proof.
   intros; subst.
   apply field_at_field_at_.
 Qed.
 
 Lemma field_at__memory_block: forall sh t gfs p,
-  field_at_ sh t gfs p =
+  field_at_ sh t gfs p ⊣⊢
   memory_block sh (sizeof (nested_field_type t gfs)) (field_address t gfs p).
 Proof.
   intros.
@@ -1021,10 +1004,10 @@ Proof.
     change (sizeof ?A) with (expr.sizeof A) in *.
     rewrite (Z.mod_small ofs) in * by lia.
     rewrite (Z.mod_small (ofs + nested_field_offset t gfs)) in H by (pose proof base.sizeof_pos (nested_field_type t gfs); lia).
-    rewrite memory_block_data_at_rec_default_val; try tauto; unfold expr.sizeof in *; try lia.
+    rewrite memory_block_data_at_rec_default_val; first done; try tauto; unfold expr.sizeof in *; try lia.
   + unfold field_at_, field_at.
     rewrite memory_block_isptr.
-    apply pred_ext; normalize.
+    apply bi.equiv_entails_2; normalize.
 Qed.
 
 Lemma mapsto_zero_data_at_zero:
@@ -1033,7 +1016,7 @@ Lemma mapsto_zero_data_at_zero:
     complete_legal_cosu_type t = true ->
     fully_nonvolatile (rank_type cenv_cs t) t = true ->
     field_compatible t nil p ->
-    mapsto_zeros (sizeof t) sh p |-- data_at sh t (zero_val t) p.
+    mapsto_zeros (sizeof t) sh p ⊢ data_at sh t (zero_val t) p.
 Proof.
 intros.
 unfold data_at, field_at.
@@ -1050,7 +1033,7 @@ rep_lia.
 Qed.
 
 Lemma data_at_data_at_ : forall sh t v p,
-  data_at sh t v p |-- data_at_ sh t p.
+  data_at sh t v p ⊢ data_at_ sh t p.
 Proof.
   intros.
   apply field_at_field_at_.
@@ -1058,15 +1041,15 @@ Qed.
 
 Lemma data_at_data_at_default : forall sh t v v' p,
   v' = default_val (nested_field_type t nil) ->
-  data_at sh t v p |-- data_at sh t v' p.
+  data_at sh t v p ⊢ data_at sh t v' p.
 Proof.
   intros; subst.
   apply data_at_data_at_.
 Qed.
 
 Lemma data_at__memory_block: forall sh t p,
-  data_at_ sh t p =
-  (!! field_compatible t nil p) && memory_block sh (sizeof t) p.
+  data_at_ sh t p ⊣⊢
+  ⌜field_compatible t nil p⌝ ∧ memory_block sh (sizeof t) p.
 Proof.
   intros.
   unfold data_at_, data_at.
@@ -1076,14 +1059,14 @@ Proof.
   + normalize.
   + unfold field_at_, field_at.
     rewrite memory_block_isptr.
-    replace (!!field_compatible t nil p : mpred) with FF by (apply ND_prop_ext; tauto).
-    replace (!!isptr Vundef : mpred) with FF by reflexivity.
-    normalize.
+    rewrite bi.pure_False by auto.
+    rewrite (bi.pure_False _ H).
+    iSplit; iIntros "([] & _)".
 Qed.
 
 Lemma memory_block_data_at_: forall sh t p,
   field_compatible t nil p ->
-  memory_block sh (sizeof t) p = data_at_ sh t p.
+  memory_block sh (sizeof t) p ⊣⊢ data_at_ sh t p.
 Proof.
   intros.
   rewrite data_at__memory_block.
@@ -1092,7 +1075,7 @@ Qed.
 
 Lemma data_at__memory_block_cancel:
    forall sh t p,
-       data_at_ sh t p |-- memory_block sh (sizeof t) p.
+       data_at_ sh t p ⊢ memory_block sh (sizeof t) p.
 Proof.
   intros.
   rewrite data_at__memory_block.
@@ -1101,33 +1084,31 @@ Qed.
 
 Lemma data_at_memory_block:
   forall sh t v p,
-     data_at sh t v p |-- memory_block sh (sizeof t) p.
+     data_at sh t v p ⊢ memory_block sh (sizeof t) p.
 Proof.
   intros.
-  eapply derives_trans; [apply data_at_data_at_; reflexivity |].
+  rewrite data_at_data_at_.
   rewrite data_at__memory_block by auto.
-  apply andp_left2.
-  auto.
+  iIntros "(_ & $)".
 Qed.
 
 Lemma array_at_array_at_: forall sh t gfs lo hi v p,
-  array_at sh t gfs lo hi v p |-- array_at_ sh t gfs lo hi p.
+  array_at sh t gfs lo hi v p ⊢ array_at_ sh t gfs lo hi p.
 Proof.
   intros.
-  eapply derives_trans; [apply andp_right; [apply array_at_local_facts | apply derives_refl] | ].
- normalize.
-  unfold array_at_.
-  apply array_at_ext_derives.
-  1: rewrite Zlength_Zrepeat by (rewrite Zlength_correct in H1; lia); lia.
+  iIntros "H".
+  iDestruct (array_at_local_facts with "H") as %H.
+  iApply (array_at_ext_derives with "H").
+  { rewrite Zlength_Zrepeat by (rewrite Zlength_correct in H; lia); lia. }
   intros.
   destruct (field_compatible0_dec t (ArraySubsc i :: gfs) p).
-  + revert u1 H5; erewrite <- @nested_field_type_ArraySubsc with (i := i); intros.
-    apply JMeq_eq in H5; rewrite H5. unfold Znth. rewrite if_false by lia.
+  + revert dependent u1; erewrite <- @nested_field_type_ArraySubsc with (i := i).
+    intros ? ->%JMeq_eq. unfold Znth. rewrite if_false by lia.
     unfold Zrepeat; rewrite nth_repeat.
     apply field_at_field_at_; auto.
   + unfold field_at.
     normalize.
-    contradiction (field_compatible_field_compatible0 t (ArraySubsc i :: gfs) p H6).
+    contradiction n; apply field_compatible_field_compatible0; done.
 Qed.
 
 Lemma withspacer_field_at__Tunion: forall sh t gfs i id a p,
@@ -1137,7 +1118,7 @@ Lemma withspacer_field_at__Tunion: forall sh t gfs i id a p,
    (nested_field_offset t gfs +
     sizeof (field_type i (co_members (get_co id))))
    (nested_field_offset t gfs + sizeof (nested_field_type t gfs))
-   (field_at_ sh t (gfs UDOT i)) p =
+   (field_at_ sh t (gfs UDOT i)) p ⊣⊢
   memory_block sh (sizeof (nested_field_type t gfs)) (field_address t gfs p).
 Proof.
   intros.
@@ -1151,7 +1132,7 @@ Proof.
     unfold field_address.
     rewrite if_false by auto.
     rewrite H.
-    apply pred_ext; normalize.
+    apply bi.equiv_entails_2; normalize.
   }
   rewrite field_at__memory_block.
   assert (field_compatible t (gfs UDOT i) p) by (rewrite field_compatible_cons, H; split; auto).
@@ -1170,8 +1151,7 @@ Proof.
   + reflexivity.
   + pose proof sizeof_pos (field_type i (co_members (get_co id))); lia.
   + lia.
-  +
-    change (sizeof ?A) with (expr.sizeof A) in *.
+  + change (sizeof ?A) with (expr.sizeof A) in *.
     split.
     - rewrite sizeof_Tunion.
       erewrite co_consistent_sizeof by apply get_co_consistent.
@@ -1201,75 +1181,49 @@ Lemma array_at_ramif: forall sh t gfs t0 n a lo hi i v v0 p,
   nested_field_type t gfs = Tarray t0 n a ->
   lo <= i < hi ->
   JMeq v0 (Znth (i - lo) v) ->
-  array_at sh t gfs lo hi v p |-- field_at sh t (ArraySubsc i :: gfs) v0 p *
-   (ALL v0: _, ALL v0': _, !! JMeq v0 v0' -->
-      (field_at sh t (ArraySubsc i :: gfs) v0 p -*
-        array_at sh t gfs lo hi (upd_Znth (i - lo) v v0') p)).
+  array_at sh t gfs lo hi v p ⊢ field_at sh t (ArraySubsc i :: gfs) v0 p ∗
+   ∀ v0 v0', ⌜JMeq v0 v0'⌝ →
+      (field_at sh t (ArraySubsc i :: gfs) v0 p -∗
+        array_at sh t gfs lo hi (upd_Znth (i - lo) v v0') p).
 Proof.
   intros.
-  rewrite (add_andp _ _ (array_at_local_facts _ _ _ _ _ _ _)).
-  normalize.
-  rewrite allp_uncurry'.
-  change (ALL  st: _,
-    !!JMeq (fst st) (snd st) -->
-     (field_at sh t (gfs SUB i) (fst st) p -*
-      array_at sh t gfs lo hi (upd_Znth (i - lo) v (snd st)) p))
-  with (allp ((fun st => !!JMeq (fst st) (snd st)) -->
-               ((fun st => field_at sh t (gfs SUB i) (fst st) p) -*
-                 fun st => array_at sh t gfs lo hi (upd_Znth (i - lo) v (snd st)) p))).
-  eapply RAMIF_Q'.solve with
-    (array_at sh t gfs lo i (sublist 0 (i - lo) v) p *
-     array_at sh t gfs (i + 1) hi (sublist (i + 1 - lo) (hi - lo) v) p).
-  + simpl; auto.
-  + erewrite (split3_array_at sh t gfs lo i hi) by (eauto; lia).
-    cancel.
-  + clear v0 H1.
-    intros [v0 v0'].
-    normalize.
-    erewrite (split3_array_at sh t gfs lo i hi).
-    2: auto.
-    2:{
-      rewrite upd_Znth_Zlength by lia.
-      auto.
-    }
-    2:{
-      rewrite upd_Znth_same by lia.
-      exact H1.
-    }
-    rewrite @sublist_upd_Znth_l with (lo := 0) by lia.
-    rewrite @sublist_upd_Znth_r with (lo := (i + 1 - lo)) by lia.
-    unfold fst; cancel.
+  iIntros "H".
+  iDestruct (array_at_local_facts with "H") as %(? & ? & ? & ?).
+  erewrite (split3_array_at sh t gfs lo i hi) by (eauto; lia).
+  iDestruct "H" as "(? & $ & ?)".
+  clear dependent v0.
+  iIntros (v0 v0' ?) "?".
+  erewrite (split3_array_at sh t gfs lo i hi).
+  2: auto.
+  2:{ rewrite upd_Znth_Zlength by lia.
+      auto. }
+  2:{ rewrite upd_Znth_same by lia.
+      done. }
+  rewrite @sublist_upd_Znth_l with (lo := 0) by lia.
+  rewrite @sublist_upd_Znth_r with (lo := (i + 1 - lo)) by lia.
+  iFrame.
 Qed.
 
 Lemma nested_sfieldlist_at_ramif: forall sh t gfs id a i v p,
   let d := default_val _ in
   nested_field_type t gfs = Tstruct id a ->
   in_members i (co_members (get_co id)) ->
-  nested_sfieldlist_at sh t gfs (co_members (get_co id)) v p |--
+  nested_sfieldlist_at sh t gfs (co_members (get_co id)) v p ⊢
   field_at sh t (StructField (name_member (get_member i (co_members (get_co id)))) :: gfs)
-    (proj_struct i (co_members (get_co id)) v d) p *
-      (ALL v0: _,
-         field_at sh t (StructField (name_member (get_member i (co_members (get_co id)))) :: gfs) v0 p -*
+    (proj_struct i (co_members (get_co id)) v d) p ∗
+      (∀ v0,
+         field_at sh t (StructField (name_member (get_member i (co_members (get_co id)))) :: gfs) v0 p -∗
            nested_sfieldlist_at sh t gfs (co_members (get_co id))
             (upd_struct i (co_members (get_co id)) v v0) p).
 Proof.
   intros.
   pose proof (get_co_members_no_replicate id).
- forget (co_members (get_co id)) as m.
- destruct m; [inv H0|].
+  forget (co_members (get_co id)) as m.
+  destruct m; [inv H0|].
   revert v d H0; intros.
   unfold nested_sfieldlist_at.
-
-  match goal with
-  | |- _ |-- _ * (ALL v0: _, ?A1 v0 p -* ?A2 (?A3 v0) p) =>
-      change (ALL v0: _, A1 v0 p -* A2 (A3 v0) p)
-      with (allp (Basics.compose (fun P => P p) (fun v0 => A1 v0) -*
-                  Basics.compose (fun v0 => A2 (A3 v0) p) (fun v0 => v0)))
-  end.
-
-  Opaque struct_pred. eapply @RAMIF_Q.trans. Transparent struct_pred.
-  2:{
-    apply (struct_pred_ramif (m::m0)
+  etrans.
+  { apply (struct_pred_ramif (m::m0)
             (fun it v p =>
               withspacer sh
                 (nested_field_offset t gfs +
@@ -1278,43 +1232,31 @@ Proof.
                 (nested_field_offset t gfs +
                  field_offset_next cenv_cs (name_member it) (m::m0)
                    (sizeof (nested_field_type t gfs)))
-                (field_at sh t (gfs DOT name_member it) v) p)); auto.
-  }
-  2:{
-    apply withspacer_ramif_Q.
-  }
-  intros.
-  apply derives_refl.
+                (field_at sh t (gfs DOT name_member it) v) p)); eauto. }
+  iIntros "(H & H1)".
+  iDestruct (withspacer_ramif_Q with "H") as "($ & H2)".
+  iIntros (?) "?"; iApply "H1"; iApply "H2"; done.
 Qed.
 
 Lemma nested_ufieldlist_at_ramif: forall sh t gfs id a i v p,
   let d := default_val _ in
   nested_field_type t gfs = Tunion id a ->
   in_members i (co_members (get_co id)) ->
-  nested_ufieldlist_at sh t gfs (co_members (get_co id)) v p |--
+  nested_ufieldlist_at sh t gfs (co_members (get_co id)) v p ⊢
   field_at sh t (UnionField (name_member (get_member i (co_members (get_co id)))) :: gfs)
-    (proj_union i (co_members (get_co id)) v d) p *
-      (ALL v0: _,
-         field_at sh t (UnionField (name_member (get_member i (co_members (get_co id)))) :: gfs) v0 p -*
+    (proj_union i (co_members (get_co id)) v d) p ∗
+      (∀ v0,
+         field_at sh t (UnionField (name_member (get_member i (co_members (get_co id)))) :: gfs) v0 p -∗
            nested_ufieldlist_at sh t gfs (co_members (get_co id))
             (upd_union i (co_members (get_co id)) v v0) p).
 Proof.
   intros.
   pose proof (get_co_members_no_replicate id).
- destruct (co_members (get_co id)) eqn:?; [inv H0|].
+  destruct (co_members (get_co id)) eqn:?; [inv H0|].
   revert v d H0; intros.
   unfold nested_ufieldlist_at.
-
-  match goal with
-  | |- _ |-- _ * (ALL v0: _, ?A1 v0 p -* ?A2 (?A3 v0) p) =>
-      change (ALL v0: _, A1 v0 p -* A2 (A3 v0) p)
-      with (allp (Basics.compose (fun P => P p) (fun v0 => A1 v0) -*
-                  Basics.compose (fun v0 => A2 (A3 v0) p) (fun v0 => v0)))
-  end.
-
-  Opaque union_pred. eapply @RAMIF_Q.trans. Transparent union_pred.
-  2:{
-    apply (union_pred_ramif (m::m0)
+  etrans.
+  { apply (union_pred_ramif (m::m0)
             (fun it v p =>
               withspacer sh
                 (nested_field_offset t gfs +
@@ -1322,33 +1264,30 @@ Proof.
                    (field_type (name_member it) (m::m0)))
                 (nested_field_offset t gfs +
                  sizeof (nested_field_type t gfs))
-                (field_at sh t (gfs UDOT name_member it) v) p)); auto.
+                (field_at sh t (gfs UDOT name_member it) v) p)); try done.
     instantiate (1 := default_val _).
     intros.
     rewrite !withspacer_spacer.
     unfold fst.
     fold (field_at_ sh t (gfs UDOT i) p).
-    eapply derives_trans; [eapply sepcon_derives; [apply derives_refl | apply field_at_field_at_] |].
+    rewrite field_at_field_at_.
     rewrite <- !withspacer_spacer.
-   rewrite name_member_get.
-   rewrite <- Heqm.
+    rewrite name_member_get.
+    rewrite <- Heqm.
     erewrite !withspacer_field_at__Tunion; try eassumption; auto.
-   rewrite name_member_get. rewrite Heqm. auto.
+    rewrite name_member_get. rewrite Heqm. auto.
     rewrite Heqm; auto.
   }
-  2:{
-    unfold fst.
-    apply withspacer_ramif_Q.
-  }
-  intros.
-  apply derives_refl.
+  iIntros "(H & H1)".
+  iDestruct (withspacer_ramif_Q with "H") as "($ & H2)".
+  iIntros (?) "?"; iApply "H1"; iApply "H2"; done.
 Qed.
 
 Lemma memory_block_valid_ptr:
   forall sh n p,
-     sepalg.nonidentity sh ->
+     sh ≠ Share.bot ->
      n > 0 ->
-     memory_block sh n p |-- valid_pointer p.
+     memory_block sh n p ⊢ valid_pointer p.
 Proof.
   intros.
   rewrite memory_block_isptr.
@@ -1364,9 +1303,9 @@ Qed.
 
 Lemma data_at__valid_ptr:
   forall sh t p,
-     sepalg.nonidentity sh ->
+     sh ≠ Share.bot ->
      sizeof t > 0 ->
-     data_at_ sh t p |-- valid_pointer p.
+     data_at_ sh t p ⊢ valid_pointer p.
 Proof.
   intros.
   rewrite data_at__memory_block.
@@ -1376,20 +1315,20 @@ Qed.
 
 Lemma data_at_valid_ptr:
   forall sh t v p,
-     sepalg.nonidentity sh ->
+     sh ≠ Share.bot ->
      sizeof t > 0 ->
-     data_at sh t v p |-- valid_pointer p.
+     data_at sh t v p ⊢ valid_pointer p.
 Proof.
   intros.
-  eapply derives_trans; [apply data_at_data_at_ |].
+  rewrite data_at_data_at_.
   apply data_at__valid_ptr; auto.
 Qed.
 
 Lemma field_at_valid_ptr:
   forall sh t path v p,
-     sepalg.nonidentity sh ->
+     sh ≠ Share.bot ->
      sizeof (nested_field_type t path) > 0 ->
-     field_at sh t path v p |-- valid_pointer (field_address t path p).
+     field_at sh t path v p ⊢ valid_pointer (field_address t path p).
 Proof.
 intros.
 rewrite field_at_data_at.
@@ -1398,10 +1337,10 @@ Qed.
 
 Lemma field_at_valid_ptr0:
   forall sh t path v p,
-     sepalg.nonidentity sh ->
+     sh ≠ Share.bot ->
      sizeof (nested_field_type t path) > 0 ->
      nested_field_offset t path = 0 ->
-     field_at sh t path v p |-- valid_pointer p.
+     field_at sh t path v p ⊢ valid_pointer p.
 Proof.
 intros.
 assert_PROP (field_compatible t path p).
@@ -1421,50 +1360,44 @@ Other lemmas
 
 ************************************************)
 
-Lemma lower_andp_val:
-  forall (P Q: val->mpred) v,
-  ((P && Q) v) = (P v && Q v).
-Proof. reflexivity. Qed.
-
-Lemma compute_legal_nested_field_spec: forall {A : Type} {ND : NatDed A} (P: A) t gfs,
-  Forall (fun Q => P |-- !!Q) (compute_legal_nested_field t gfs) ->
-  P |-- !! (legal_nested_field t gfs).
+Lemma compute_legal_nested_field_spec: forall (P: mpred) t gfs,
+  Forall (fun Q => P ⊢ ⌜Q⌝) (compute_legal_nested_field t gfs) ->
+  P ⊢ ⌜legal_nested_field t gfs⌝.
 Proof.
   intros.
   induction gfs as [| gf gfs].
   + simpl.
-    apply prop_right; auto.
+    by iIntros "?".
   + simpl in H |- *.
     unfold legal_field.
     destruct (nested_field_type t gfs), gf; inversion H; subst;
     try
     match goal with
-    | HH : P |-- (prop False) |-
-           P |-- (prop (_)) => apply (derives_trans _ _ _ HH); apply prop_derives; tauto
+    | HH : P ⊢ ⌜False⌝ |-
+           P ⊢ ⌜_⌝ => rewrite HH; apply bi.pure_mono; tauto
     end.
     - apply IHgfs in H3.
       rewrite (add_andp _ _ H2).
       rewrite (add_andp _ _ H3).
       normalize.
-      apply prop_right; tauto.
     - destruct_in_members i0 (co_members (get_co i)).
-      * apply IHgfs in H.
-        apply (derives_trans _ _ _ H), prop_derives; tauto.
+      * apply IHgfs in H as ->.
+        apply bi.pure_mono; tauto.
       * inversion H1.
     - destruct_in_members i0 (co_members (get_co i)).
-      * apply IHgfs in H.
-        apply (derives_trans _ _ _ H), prop_derives; tauto.
-      * inversion H.
-        apply (derives_trans _ _ _ H6), prop_derives; tauto.
+      * apply IHgfs in H as ->.
+        apply bi.pure_mono; tauto.
+      * inv H.
+        rewrite H6; iIntros "[]".
     - destruct_in_members i0 (co_members (get_co i)).
-      * apply IHgfs in H.
-        apply (derives_trans _ _ _ H), prop_derives; tauto.
+      * apply IHgfs in H as ->.
+        apply bi.pure_mono; tauto.
       * inversion H1.
     - destruct_in_members i0 (co_members (get_co i)).
-      * apply IHgfs in H.
-        apply (derives_trans _ _ _ H), prop_derives; tauto.
-      * inversion H.
-        apply (derives_trans _ _ _ H6), prop_derives; tauto.
+      * apply IHgfs in H as ->.
+        apply bi.pure_mono; tauto.
+      * inv H.
+        rewrite H6; iIntros "[]".
 Qed.
 
 
@@ -1476,7 +1409,7 @@ Proof.
   intros.
   induction gfs as [| gf gfs].
   + simpl; auto.
-  +  simpl in H|-*.
+  + simpl in H|-*.
     unfold legal_field. unfold nested_field_type in *.
     destruct (nested_field_rec t gfs) as [[? ?] | ].
     destruct t0; try now inv H; contradiction.
@@ -1503,10 +1436,10 @@ Definition compute_legal_nested_field0 (t: type) (gfs: list gfield) : list Prop 
     | Tarray _ n _, ArraySubsc i =>
        (0 <= i <= n) :: compute_legal_nested_field t gfs0
     | Tstruct id _, StructField i =>
-       if compute_in_members i (co_members (get_co id)) then compute_legal_nested_field t gfs else False :: nil
+       if compute_in_members i (co_members (get_co id)) then compute_legal_nested_field t gfs else False%type :: nil
     | Tunion id _, UnionField i =>
-       if compute_in_members i (co_members (get_co id)) then compute_legal_nested_field t gfs else False :: nil
-    | _, _ => False :: nil
+       if compute_in_members i (co_members (get_co id)) then compute_legal_nested_field t gfs else False%type :: nil
+    | _, _ => False%type :: nil
     end
   end.
 
@@ -1552,59 +1485,51 @@ erewrite Share.split_together; eauto.
 Qed.
 
 Lemma field_at_conflict: forall sh t fld p v v',
-  sepalg.nonidentity sh ->
+  sh ≠ Share.bot ->
   0 < sizeof (nested_field_type t fld) ->
-  field_at sh t fld v p * field_at sh t fld v' p|-- FF.
+  field_at sh t fld v p ∗ field_at sh t fld v' p ⊢ False.
 Proof.
   intros.
-  rewrite field_at_compatible'. normalize.
-  destruct H1 as [? [? [? [? ?]]]].
-  destruct (nested_field_offset_in_range t fld H5 H2).
+  rewrite field_at_compatible'.
+  iIntros "(((% & % & % & % & %) & ?) & ?)".
+  destruct (nested_field_offset_in_range t fld); [done..|].
   assert (0 < sizeof (nested_field_type t fld) < Ptrofs.modulus).
   {
-    destruct p; inv H1.
-    simpl in H3.
+    destruct p; try done.
+    simpl in *.
     inv_int i.
     unfold expr.sizeof in *.
     lia.
   }
-  clear - H H1 H8.
-  eapply derives_trans.
-  + apply sepcon_derives.
-    apply field_at_field_at_; try assumption; auto.
-    apply field_at_field_at_; try assumption; auto.
-  + fold (field_at_ sh t fld p).
-    rewrite field_at__memory_block by auto.
-    normalize.
-    apply memory_block_conflict; try  (unfold Ptrofs.max_unsigned; lia).
-    apply sepalg.nonidentity_nonunit; auto.
+  rewrite !field_at_field_at_.
+  rewrite field_at__memory_block by auto.
+  iApply (memory_block_conflict with "[$]"); try (unfold Ptrofs.max_unsigned; lia).
 Qed.
 
 Lemma data_at_conflict: forall sh t v v' p,
-  sepalg.nonidentity sh ->
+  sh ≠ Share.bot ->
   0 < sizeof t ->
-  data_at sh t v p * data_at sh t v' p |-- FF.
+  data_at sh t v p ∗ data_at sh t v' p ⊢ False.
 Proof.
   intros. unfold data_at. apply field_at_conflict; auto.
 Qed.
 
 Lemma field_at__conflict:
   forall sh t fld p,
-  sepalg.nonidentity sh ->
+  sh ≠ Share.bot ->
   0 < sizeof (nested_field_type t fld) ->
         field_at_ sh t fld p
-        * field_at_ sh t fld p |-- FF.
+        ∗ field_at_ sh t fld p ⊢ False.
 Proof.
 intros.
 apply field_at_conflict; auto.
 Qed.
 
-Lemma sepcon_FF_derives':
-  forall (P Q: mpred), (Q |-- FF) -> P * Q |-- FF.
+Lemma sepcon_False_derives':
+  forall (P Q: mpred), (Q ⊢ False) -> P ∗ Q ⊢ False.
 Proof.
-intros.
-eapply derives_trans. apply sepcon_derives; try eassumption; eauto.
-rewrite sepcon_FF. auto.
+  intros ?? ->.
+  iIntros "(_ & [])".
 Qed.
 
 Lemma field_compatible_offset_isptr:
@@ -1663,21 +1588,21 @@ Lemma var_block_data_at_:
   Z.ltb (sizeof t) Ptrofs.modulus = true ->
   is_aligned cenv_cs ha_env_cs la_env_cs t 0 = true ->
   readable_share sh ->
-  var_block sh (id, t) = `(data_at_ sh t) (eval_lvar id t).
+  var_block sh (id, t) ⊣⊢ assert_of (`(data_at_ sh t) (eval_lvar id t)).
 Proof.
-  intros; extensionality rho.
-  unfold var_block.
-  unfold_lift.
-  simpl.
+  intros; split => rho.
+  unfold var_block; monPred.unseal.
+  unfold_lift; simpl.
   apply Zlt_is_lt_bool in H0.
   rewrite data_at__memory_block; try auto.
   rewrite memory_block_isptr.
   unfold local, lift1; unfold_lift.
   pose proof eval_lvar_spec id t rho.
   destruct (eval_lvar id t rho); simpl in *; normalize.
+  { iSplit; iIntros "((_ & []) & _)". }
   subst.
-  f_equal.
-  apply ND_prop_ext.
+  apply bi.and_proper; last done.
+  apply bi.pure_iff.
   unfold field_compatible.
   unfold isptr, legal_nested_field, size_compatible, align_compatible.
   change (Ptrofs.unsigned Ptrofs.zero) with 0.
@@ -1687,63 +1612,59 @@ Proof.
   apply la_env_cs_sound in H1; tauto.
 Qed.
 
-End CENV.
-
-#[export] Hint Extern 2 (memory_block _ _ _ |-- valid_pointer _) =>
-  (apply memory_block_valid_ptr; [auto with valid_pointer | rep_lia]) : valid_pointer.
-
 Lemma valid_pointer_weak:
- forall a, valid_pointer a |-- weak_valid_pointer a.
+ forall a, valid_pointer a ⊢ weak_valid_pointer a.
 Proof.
 intros.
 unfold valid_pointer, weak_valid_pointer.
-change predicates_hered.orp with orp.
-apply orp_right1.
-auto.
+iIntros "$".
 Qed.
 
 Lemma valid_pointer_weak':
-  forall P q, (P |-- valid_pointer q) ->
-                 P |-- weak_valid_pointer q.
+  forall P q, (P ⊢ valid_pointer q) ->
+                 P ⊢ weak_valid_pointer q.
 Proof.
 intros.
-eapply derives_trans; try eassumption.
-apply valid_pointer_weak.
+rewrite <- valid_pointer_weak; done.
 Qed.
 
-#[export] Hint Resolve valid_pointer_weak' : valid_pointer.
-
 Lemma valid_pointer_offset_zero: forall P q,
-   (P |-- valid_pointer (offset_val 0 q)) ->
-   P |-- valid_pointer q.
+   (P ⊢ valid_pointer (offset_val 0 q)) ->
+   P ⊢ valid_pointer q.
 Proof.
 intros.
 destruct q; auto.
-eapply derives_trans; try eassumption.
-simpl valid_pointer.
-constructor.
-intros ? ?. contradiction H0.
-rewrite offset_val_zero_Vptr in H.
-auto.
+- rewrite H.
+  simpl valid_pointer.
+  iIntros "[]".
+- rewrite offset_val_zero_Vptr in H.
+  auto.
 Qed.
 
-#[export] Hint Extern 1 (_ |-- valid_pointer ?Q) =>
+End CENV.
+
+#[export] Hint Extern 2 (memory_block _ _ _ ⊢ valid_pointer _) =>
+  (apply memory_block_valid_ptr; [auto with valid_pointer | rep_lia]) : valid_pointer.
+
+#[export] Hint Resolve valid_pointer_weak' : valid_pointer.
+
+#[export] Hint Extern 1 (_ ⊢ valid_pointer ?Q) =>
   lazymatch Q with
   | offset_val _ _ => fail
   | _ => apply valid_pointer_offset_zero
   end : core.
 
-#[export] Hint Extern 2 (memory_block _ _ _ |-- weak_valid_pointer _) =>
-  (apply SeparationLogic.memory_block_weak_valid_pointer;
+#[export] Hint Extern 2 (memory_block _ _ _ ⊢ weak_valid_pointer _) =>
+  (apply memory_block_weak_valid_pointer;
         [rep_lia | rep_lia | auto with valid_pointer]) : valid_pointer.
 
 Ltac field_at_conflict z fld :=
-eapply derives_trans with FF; [ | apply FF_left];
- rewrite <- ?sepcon_assoc;
+trans False; [ | apply bi.False_elim];
+ rewrite ?bi.sep_assoc;
  unfold data_at_, data_at, field_at_;
  let x := fresh "x" in set (x := field_at _ _ fld _ z); pull_right x;
  let y := fresh "y" in set (y := field_at _ _ fld _ z); pull_right y;
- try (rewrite sepcon_assoc; eapply sepcon_FF_derives');
+ try (rewrite <- bi.sep_assoc; eapply sepcon_False_derives');
  subst x y;
  apply field_at_conflict; auto;
  try solve [simpl;  (* This simpl seems safe enough, it's just simplifying (sizeof (nested_field_type _ _))
@@ -1759,15 +1680,15 @@ Ltac data_at_conflict_neq_aux1 A sh fld E x y :=
    | context [field_at sh _ fld _ y] => idtac
    | context [field_at_ sh _ fld y]  => idtac
    end;
-   apply derives_trans with (!! (~ E) && A);
-   [apply andp_right; [ | apply derives_refl];
+   trans (⌜~ E⌝ ∧ A);
+   [apply bi.and_intro; [ | apply derives_refl];
     let H := fresh in
     apply not_prop_right; intro H;
     (rewrite H || rewrite (ptr_eq_e _ _ H));
     field_at_conflict y fld
-   | apply derives_extract_prop;
+   | apply bi.pure_elim_l;
      let H1 := fresh in intro H1;
-     rewrite (eq_True _ H1)
+     rewrite (bi.pure_True _ H1)
     ].
 
 Ltac data_at_conflict_neq_aux2 A E x y :=
@@ -1779,7 +1700,7 @@ Ltac data_at_conflict_neq_aux2 A E x y :=
    end.
 
 Ltac data_at_conflict_neq :=
-  match goal with |- ?A |-- ?B =>
+  match goal with |- ?A ⊢ ?B =>
    match B with
    | context [?x <> ?y] => data_at_conflict_neq_aux2 A (x=y) x y
    | context [~ ptr_eq ?x ?y] => data_at_conflict_neq_aux2 A (ptr_eq x y) x y
@@ -1846,33 +1767,39 @@ Qed.
  (apply malloc_compatible_field_compatible;
   [assumption | reflexivity | reflexivity]) : core.
 
+Section local_facts.
+
+Context `{!heapGS Σ}.
+
 Lemma data_array_at_local_facts {cs: compspecs}:
  forall t' n a sh (v: list (reptype t')) p,
-  data_at sh (Tarray t' n a) v p |--
-  !! (field_compatible (Tarray t' n a) nil p
+  data_at sh (Tarray t' n a) v p ⊢
+  ⌜field_compatible (Tarray t' n a) nil p
      /\ Zlength v = Z.max 0 n
-     /\ Forall (value_fits t') v).
+     /\ Forall (value_fits t') v⌝.
 Proof.
 intros.
-eapply derives_trans; [apply data_at_local_facts |].
-apply prop_derives.
+rewrite data_at_local_facts.
+apply bi.pure_mono.
 intros [? ?]; split; auto.
 Qed.
 
 Lemma data_array_at_local_facts' {cs: compspecs}:
  forall t' n a sh (v: list (reptype t')) p,
   n >= 0 ->
-  data_at sh (Tarray t' n a) v p |--
-  !! (field_compatible (Tarray t' n a) nil p
+  data_at sh (Tarray t' n a) v p ⊢
+  ⌜field_compatible (Tarray t' n a) nil p
      /\ Zlength v = n
-     /\ Forall (value_fits t') v).
+     /\ Forall (value_fits t') v⌝.
 Proof.
 intros.
-eapply derives_trans; [apply data_array_at_local_facts |].
-apply prop_derives.
+rewrite data_array_at_local_facts.
+apply bi.pure_mono.
 intros [? [? ?]]; split3; auto.
 rewrite Z.max_r in H1 by lia. auto.
 Qed.
+
+End local_facts.
 
 Lemma value_fits_by_value {cs: compspecs}:
   forall t v,
@@ -1887,8 +1814,8 @@ Qed.
 
 Ltac field_at_saturate_local :=
 unfold data_at;
-match goal with |- field_at ?sh ?t ?path ?v ?c |-- _ =>
-eapply derives_trans; [apply field_at_local_facts |];
+match goal with |- field_at ?sh ?t ?path ?v ?c ⊢ _ =>
+rewrite field_at_local_facts;
   let p := fresh "p" in set (p := nested_field_type t path);
   simpl in p; unfold field_type in p; simpl in p; subst p;  (* these simpls are probably not dangerous *)
   try rewrite value_fits_by_value by reflexivity;
@@ -1901,35 +1828,35 @@ end.
 Ltac data_at_valid_aux :=
  first [computable | unfold sizeof; simpl Ctypes.sizeof; rewrite ?Z.max_r by rep_lia; rep_lia | rep_lia].
 
-#[export] Hint Extern 1 (data_at _ _ _ _ |-- valid_pointer _) =>
+#[export] Hint Extern 1 (data_at _ _ _ _ ⊢ valid_pointer _) =>
     (simple apply data_at_valid_ptr; [now auto | data_at_valid_aux]) : valid_pointer.
 
-#[export] Hint Extern 1 (field_at _ _ _ _ _ |-- valid_pointer _) =>
+#[export] Hint Extern 1 (field_at _ _ _ _ _ ⊢ valid_pointer _) =>
     (simple apply field_at_valid_ptr; [now auto | data_at_valid_aux]) : valid_pointer.
 
-#[export] Hint Extern 1 (data_at_ _ _ _ |-- valid_pointer _) =>
+#[export] Hint Extern 1 (data_at_ _ _ _ ⊢ valid_pointer _) =>
     (simple apply data_at__valid_ptr; [now auto | data_at_valid_aux]) : valid_pointer.
 
-#[export] Hint Extern 1 (field_at_ _ _ _ _ |-- valid_pointer _) =>
+#[export] Hint Extern 1 (field_at_ _ _ _ _ ⊢ valid_pointer _) =>
     (apply field_at_valid_ptr; [now auto | data_at_valid_aux]) : valid_pointer.
 
-#[export] Hint Extern 1 (field_at _ _ _ _ _ |-- _) =>
+#[export] Hint Extern 1 (field_at _ _ _ _ _ ⊢ _) =>
  (field_at_saturate_local) : saturate_local.
 
-#[export] Hint Extern 1 (data_at _ _ _ _ |-- _) =>
+#[export] Hint Extern 1 (data_at _ _ _ _ ⊢ _) =>
  (field_at_saturate_local) : saturate_local.
 
 #[export] Hint Resolve array_at_local_facts array_at__local_facts : saturate_local.
 
 #[export] Hint Resolve field_at__local_facts : saturate_local.
 #[export] Hint Resolve data_at__local_facts : saturate_local.
-#[export] Hint Extern 0 (data_at _ (Tarray _ _ _) _ _ |-- _) =>
+#[export] Hint Extern 0 (data_at _ (Tarray _ _ _) _ _ ⊢ _) =>
   (apply data_array_at_local_facts'; lia) : saturate_local.
-#[export] Hint Extern 0 (data_at _ (tarray _ _) _ _ |-- _) =>
+#[export] Hint Extern 0 (data_at _ (tarray _ _) _ _ ⊢ _) =>
   (apply data_array_at_local_facts'; lia) : saturate_local.
-#[export] Hint Extern 1 (data_at _ (Tarray _ _ _) _ _ |-- _) =>
+#[export] Hint Extern 1 (data_at _ (Tarray _ _ _) _ _ ⊢ _) =>
   (apply data_array_at_local_facts) : saturate_local.
-#[export] Hint Extern 1 (data_at _ (tarray _ _) _ _ |-- _) =>
+#[export] Hint Extern 1 (data_at _ (tarray _ _) _ _ ⊢ _) =>
   (apply data_array_at_local_facts) : saturate_local.
 #[export] Hint Rewrite <- @field_at_offset_zero: norm1.
 #[export] Hint Rewrite <- @field_at__offset_zero: norm1.
@@ -1945,65 +1872,71 @@ Ltac data_at_valid_aux :=
   as Hint Resolve derives_refl, to limit their application
   and make them fail faster *)
 
+Section cancel.
+
+Context `{!heapGS Σ}.
+
 Lemma data_at_cancel:
   forall {cs: compspecs} sh t v p,
-    data_at sh t v p |-- data_at sh t v p.
+    data_at sh t v p ⊢ data_at sh t v p.
 Proof. intros. apply derives_refl. Qed.
 Lemma field_at_cancel:
   forall {cs: compspecs} sh t gfs v p,
-    field_at sh t gfs v p |-- field_at sh t gfs v p.
+    field_at sh t gfs v p ⊢ field_at sh t gfs v p.
 Proof. intros. apply derives_refl. Qed.
 
 Lemma data_at_field_at_cancel:
   forall {cs: compspecs} sh t v p,
-    data_at sh t v p |-- field_at sh t nil v p.
+    data_at sh t v p ⊢ field_at sh t nil v p.
 Proof. intros. apply derives_refl. Qed.
 Lemma field_at_data_at_cancel:
   forall {cs: compspecs} sh t v p,
-    field_at sh t nil v p |-- data_at sh t v p.
+    field_at sh t nil v p ⊢ data_at sh t v p.
 Proof. intros. apply derives_refl. Qed.
-
-#[export] Hint Resolve data_at_cancel field_at_cancel
-   data_at_field_at_cancel field_at_data_at_cancel : cancel.
 
 Lemma field_at__data_at__cancel:
   forall {cs: compspecs} sh t p,
-   field_at_ sh t nil p |-- data_at_ sh t p.
+   field_at_ sh t nil p ⊢ data_at_ sh t p.
 Proof. intros. apply derives_refl. Qed.
 
 Lemma data_at__field_at__cancel:
   forall {cs: compspecs} sh t p,
-   data_at_ sh t p |-- field_at_ sh t nil p.
+   data_at_ sh t p ⊢ field_at_ sh t nil p.
 Proof. intros. apply derives_refl. Qed.
-#[export] Hint Resolve  field_at__data_at__cancel data_at__field_at__cancel : cancel.
 
+End cancel.
+
+#[export] Hint Resolve data_at_cancel field_at_cancel
+   data_at_field_at_cancel field_at_data_at_cancel : cancel.
+
+#[export] Hint Resolve  field_at__data_at__cancel data_at__field_at__cancel : cancel.
 
 (* We do these as Hint Extern, instead of Hint Resolve,
   to limit their application and make them fail faster *)
 
-#[export] Hint Extern 2 (field_at _ _ _ _ _ |-- field_at_ _ _ _ _) =>
+#[export] Hint Extern 2 (field_at _ _ _ _ _ ⊢ field_at_ _ _ _ _) =>
    (simple apply field_at_field_at_) : cancel.
 
-#[export] Hint Extern 2 (field_at _ _ _ _ _ |-- field_at _ _ _ _ _) =>
+#[export] Hint Extern 2 (field_at _ _ _ _ _ ⊢ field_at _ _ _ _ _) =>
   (simple apply field_at_field_at_default;
    match goal with |- _ = default_val _ => reflexivity end) : cancel.
 
-#[export] Hint Extern 1 (data_at _ _ _ _ |-- data_at_ _ _ _) =>
+#[export] Hint Extern 1 (data_at _ _ _ _ ⊢ data_at_ _ _ _) =>
     (simple apply data_at_data_at_) : cancel.
 
-#[export] Hint Extern 1 (data_at _ _ _ _ |-- memory_block _ _ _) =>
+#[export] Hint Extern 1 (data_at _ _ _ _ ⊢ memory_block _ _ _) =>
     (simple apply data_at__memory_block_cancel) : cancel.
 
-#[export] Hint Extern 2 (data_at _ _ _ _ |-- data_at _ _ _ _) =>
+#[export] Hint Extern 2 (data_at _ _ _ _ ⊢ data_at _ _ _ _) =>
   (simple apply data_at_data_at_default;
    match goal with |- _ = default_val _ => reflexivity end) : cancel.
 
 (* too slow this way.
-#[export] Hint Extern 2 (data_at _ _ _ _ |-- data_at _ _ _ _) =>
+#[export] Hint Extern 2 (data_at _ _ _ _ ⊢ data_at _ _ _ _) =>
   (apply data_at_data_at_default; reflexivity) : cancel.
 *)
 
-#[export] Hint Extern 2 (array_at _ _ _ _ _ _ _ |-- array_at_ _ _ _ _ _ _) =>
+#[export] Hint Extern 2 (array_at _ _ _ _ _ _ _ ⊢ array_at_ _ _ _ _ _ _) =>
   (simple apply array_at_array_at_) : cancel.
 #[export] Hint Extern 1 (isptr _) => (eapply field_compatible_offset_isptr; eassumption) : core.
 #[export] Hint Extern 1 (isptr _) => (eapply field_compatible0_offset_isptr; eassumption) : core.
@@ -2071,58 +2004,61 @@ Ltac find_data_at N :=
 Definition protect (T: Type) (x: T) := x.
 Global Opaque protect.
 
-Lemma field_at_ptr_neq{cs: compspecs} :
+Section lemmas.
+
+Context `{!heapGS Σ}.
+
+Lemma field_at_ptr_neq {cs: compspecs} :
    forall sh t fld p1 p2 v1 v2,
-  sepalg.nonidentity sh ->
+  sh ≠ Share.bot ->
    0 < sizeof (nested_field_type t (fld :: nil))  ->
-   field_at sh t (fld::nil) v1 p1 *
+   field_at sh t (fld::nil) v1 p1 ∗
    field_at sh t (fld::nil) v2 p2
-   |--
-   !! (~ ptr_eq p1 p2).
+   ⊢
+   ⌜~ ptr_eq p1 p2⌝.
 Proof.
    intros.
    apply not_prop_right; intros.
-  rewrite -> (ptr_eq_e _ _ H1).
+   rewrite -> (ptr_eq_e _ _ H1).
    apply field_at_conflict; try assumption.
 Qed.
 
-Lemma field_at_ptr_neq_andp_emp{cs: compspecs} :
+Lemma field_at_ptr_neq_andp_emp {cs: compspecs} :
     forall sh t fld p1 p2 v1 v2,
-  sepalg.nonidentity sh ->
+  sh ≠ Share.bot ->
  0 < sizeof (nested_field_type t (fld :: nil))  ->
-   field_at sh t (fld::nil) v1 p1 *
+   field_at sh t (fld::nil) v1 p1 ∗
    field_at sh t (fld::nil) v2 p2
-   |--
-   field_at sh t (fld::nil) v1 p1 *
-   field_at sh t (fld::nil) v2 p2 *
-   (!! (~ ptr_eq p1 p2) && emp).
+   ⊢
+   field_at sh t (fld::nil) v1 p1 ∗
+   field_at sh t (fld::nil) v2 p2 ∗
+   (⌜~ ptr_eq p1 p2⌝ ∧ emp).
 Proof.
-   intros.
-   normalize.
-   apply andp_right.
-   apply field_at_ptr_neq; assumption.
-   cancel.
+  intros.
+  iIntros "H".
+  iDestruct (field_at_ptr_neq with "H") as %?.
+  iDestruct "H" as "($ & $)"; done.
 Qed.
 
-Lemma field_at_ptr_neq_null{cs: compspecs} :
+Lemma field_at_ptr_neq_null {cs: compspecs} :
    forall sh t fld v p,
-   field_at sh t fld v p |-- !! (~ ptr_eq p nullval).
+   field_at sh t fld v p ⊢ ⌜~ ptr_eq p nullval⌝.
 Proof.
-   intros.
-   rewrite -> field_at_isptr.
-  normalize. apply prop_right.
-   destruct p; unfold nullval; simpl in *; tauto.
+  intros.
+  rewrite -> field_at_isptr.
+  normalize. apply bi.pure_intro.
+  destruct p; unfold nullval; simpl in *; tauto.
 Qed.
 
 Lemma spacer_share_join:
   forall sh1 sh2 sh J K q,
    sepalg.join sh1 sh2 sh ->
-   spacer sh1 J K q * spacer sh2 J K q = spacer sh J K q.
+   spacer sh1 J K q ∗ spacer sh2 J K q ⊣⊢ spacer sh J K q.
 Proof.
- intros.
- unfold spacer.
-  if_tac. normalize.
- unfold at_offset.
+  intros.
+  unfold spacer.
+  if_tac. { apply bi.sep_emp. }
+  unfold at_offset.
   apply memory_block_share_join; auto.
 Qed.
 
@@ -2132,11 +2068,10 @@ Lemma struct_pred_cons2:
    (v: compact_prod (map A (it::it'::m)))
    (p: val),
  struct_pred (it :: it' :: m) P v p =
-    P _ (fst v) p * struct_pred (it'::m) P (snd v) p.
+    (P _ (fst v) p ∗ struct_pred (it'::m) P (snd v) p).
 Proof.
 intros.
-destruct v. unfold fst, snd.
-reflexivity.
+destruct v; reflexivity.
 Qed.
 
 Lemma union_pred_cons2:
@@ -2153,15 +2088,15 @@ Qed.
 
 Lemma data_at_rec_void:
   forall {cs: compspecs}
-      sh t v q, t = Tvoid -> data_at_rec sh t v q = FF.
+      sh t v q, t = Tvoid -> data_at_rec sh t v q = False.
 Proof.
  intros; subst; reflexivity.
 Qed.
 
-Lemma field_at_share_join{cs: compspecs}:
+Lemma field_at_share_join {cs: compspecs}:
   forall sh1 sh2 sh t gfs v p,
     sepalg.join sh1 sh2 sh ->
-   field_at sh1 t gfs v p * field_at sh2 t gfs v p = field_at sh t gfs v p.
+   field_at sh1 t gfs v p ∗ field_at sh2 t gfs v p ⊣⊢ field_at sh t gfs v p.
 Proof.
 intros.
 unfold field_at.
@@ -2175,22 +2110,22 @@ destruct p; try inversion H1.
 apply data_at_rec_share_join; auto.
 Qed.
 
-Lemma field_at__share_join{cs: compspecs}:
+Lemma field_at__share_join {cs: compspecs}:
   forall sh1 sh2 sh t gfs p,
     sepalg.join sh1 sh2 sh ->
-   field_at_ sh1 t gfs p * field_at_ sh2 t gfs p = field_at_ sh t gfs p.
+   field_at_ sh1 t gfs p ∗ field_at_ sh2 t gfs p ⊣⊢ field_at_ sh t gfs p.
 Proof. intros. apply field_at_share_join. auto. Qed.
 
-Lemma data_at_share_join{cs: compspecs}:
+Lemma data_at_share_join {cs: compspecs}:
   forall sh1 sh2 sh t v p,
     sepalg.join sh1 sh2 sh ->
-   data_at sh1 t v p * data_at sh2 t v p = data_at sh t v p.
+   data_at sh1 t v p ∗ data_at sh2 t v p ⊣⊢ data_at sh t v p.
 Proof. intros. apply field_at_share_join; auto. Qed.
 
-Lemma data_at__share_join{cs: compspecs}:
+Lemma data_at__share_join {cs: compspecs}:
   forall sh1 sh2 sh t p,
     sepalg.join sh1 sh2 sh ->
-   data_at_ sh1 t p * data_at_ sh2 t p = data_at_ sh t p.
+   data_at_ sh1 t p ∗ data_at_ sh2 t p ⊣⊢ data_at_ sh t p.
 Proof. intros. apply data_at_share_join; auto. Qed.
 
 Lemma nonreadable_memory_block_field_at:
@@ -2198,7 +2133,7 @@ Lemma nonreadable_memory_block_field_at:
       sh t gfs v p,
   ~ readable_share sh ->
    value_fits _ v ->
-   memory_block sh (sizeof (nested_field_type t gfs)) (field_address t gfs p) = field_at sh t gfs v p.
+   memory_block sh (sizeof (nested_field_type t gfs)) (field_address t gfs p) ⊣⊢ field_at sh t gfs v p.
 Proof.
   intros until p. intros NONREAD VF.
   unfold field_address.
@@ -2226,14 +2161,14 @@ Proof.
     apply nonreadable_memory_block_data_at_rec; try tauto; try lia.
   + unfold field_at_, field_at.
     rewrite memory_block_isptr.
-    apply pred_ext; normalize.
+    apply bi.equiv_entails_2; normalize.
 Qed.
 
-Lemma nonreadable_memory_block_data_at: forall  {cs: compspecs} sh t v p,
+Lemma nonreadable_memory_block_data_at: forall {cs: compspecs} sh t v p,
   ~ readable_share sh ->
   field_compatible t nil p ->
   value_fits t v ->
-  memory_block sh (sizeof t) p = data_at sh t v p.
+  memory_block sh (sizeof t) p ⊣⊢ data_at sh t v p.
 Proof.
   intros.
   replace p with (field_address t nil p) at 1.
@@ -2250,11 +2185,11 @@ Lemma nonreadable_field_at_eq {cs: compspecs} :
   forall sh t gfs v v' p,
    ~ readable_share sh ->
    (value_fits (nested_field_type t gfs) v <-> value_fits (nested_field_type t gfs) v') ->
-   field_at sh t gfs v p = field_at sh t gfs v' p.
+   field_at sh t gfs v p ⊣⊢ field_at sh t gfs v' p.
 Proof.
 intros.
 rewrite !field_at_data_at.
-apply pred_ext; saturate_local.
+apply bi.equiv_entails_2; saturate_local.
 rewrite <- !nonreadable_memory_block_data_at; auto.
 apply H0; auto.
 destruct (readable_share_dec sh); try contradiction.
@@ -2267,23 +2202,22 @@ Lemma nonreadable_readable_memory_block_data_at_join
   forall ash bsh psh t v p,
     sepalg.join ash bsh psh ->
     ~ readable_share ash ->
-   memory_block ash (sizeof t) p * data_at bsh t v p = data_at psh t v p.
+   memory_block ash (sizeof t) p ∗ data_at bsh t v p ⊣⊢ data_at psh t v p.
 Proof.
 intros.
-apply pred_ext; saturate_local.
-rewrite @nonreadable_memory_block_data_at with (v:=v); auto.
-unfold data_at.
-erewrite field_at_share_join; eauto. apply derives_refl.
+apply bi.equiv_entails_2; saturate_local.
 rewrite @nonreadable_memory_block_data_at with (v:=v); auto.
 unfold data_at.
 erewrite field_at_share_join; eauto.
-apply derives_refl.
+rewrite @nonreadable_memory_block_data_at with (v:=v); auto.
+unfold data_at.
+erewrite field_at_share_join; eauto.
 Qed.
 
 Lemma nonreadable_data_at_eq {cs: compspecs}:
   forall sh t v v' p, ~readable_share sh ->
    (value_fits t v <-> value_fits t v') ->
-     data_at sh t v p = data_at sh t v' p.
+     data_at sh t v p ⊣⊢ data_at sh t v' p.
 Proof.
 intros.
 unfold data_at.
@@ -2294,7 +2228,7 @@ Lemma field_at_share_join_W {cs: compspecs}:
   forall sh1 sh2 sh t gfs v1 v2 p,
     sepalg.join sh1 sh2 sh ->
     writable_share sh1 ->
-    field_at sh1 t gfs v1 p * field_at sh2 t gfs v2 p |-- field_at sh t gfs v1 p.
+    field_at sh1 t gfs v1 p ∗ field_at sh2 t gfs v2 p ⊢ field_at sh t gfs v1 p.
 Proof.
   intros.
   pose proof join_writable_readable H H0.
@@ -2310,7 +2244,7 @@ Lemma data_at_share_join_W {cs: compspecs}:
   forall sh1 sh2 sh t v1 v2 p,
     sepalg.join sh1 sh2 sh ->
     writable_share sh1 ->
-    data_at sh1 t v1 p * data_at sh2 t v2 p |-- data_at sh t v1 p.
+    data_at sh1 t v1 p ∗ data_at sh2 t v2 p ⊢ data_at sh t v1 p.
 Proof.
   intros.
   apply field_at_share_join_W; auto.
@@ -2321,18 +2255,19 @@ Lemma value_fits_Tint_trivial {cs: compspecs} :
 Proof.
 intros.
 rewrite value_fits_eq; simpl.
+unfold type_is_volatile; simpl.
 destruct (attr_volatile a); auto.
 hnf. intro. apply Coq.Init.Logic.I.
 Qed.
 
 (* TODO: move all change type lemmas into one file. Also those change compspecs lemmas. *)
-Lemma data_at_tuint_tint {cs: compspecs}: forall sh v p, data_at sh tuint v p = data_at sh tint v p.
+Lemma data_at_tuint_tint {cs: compspecs}: forall sh v p, data_at sh tuint v p ⊣⊢ data_at sh tint v p.
 Proof.
   intros.
   unfold data_at, field_at.
-  f_equal.
+  apply bi.and_proper; last done.
   unfold field_compatible.
-  apply ND_prop_ext.
+  apply bi.pure_iff.
   assert (align_compatible tuint p <-> align_compatible tint p); [| tauto].
   destruct p; simpl; try tauto.
   split; intros.
@@ -2349,7 +2284,7 @@ Lemma mapsto_field_at {cs: compspecs} sh t gfs v v' p:
   type_is_volatile (nested_field_type t gfs) = false ->
   field_compatible t gfs p ->
   JMeq v v' ->
-  mapsto sh (nested_field_type t gfs) (field_address t gfs p) v = field_at sh t gfs v' p.
+  mapsto sh (nested_field_type t gfs) (field_address t gfs p) v ⊣⊢ field_at sh t gfs v' p.
 Proof.
   intros.
   unfold field_at, at_offset.
@@ -2357,7 +2292,7 @@ Proof.
   apply (fun HH => JMeq_trans HH (JMeq_sym (repinject_JMeq _ v' H))) in H2.
   apply JMeq_eq in H2.
   rewrite prop_true_andp by auto.
-  f_equal; auto.
+  f_equiv; auto.
   apply field_compatible_field_address; auto.
 Qed.
 
@@ -2366,9 +2301,9 @@ Lemma mapsto_field_at_ramify {cs: compspecs} sh t gfs v v' w w' p:
   type_is_volatile (nested_field_type t gfs) = false ->
   JMeq v v' ->
   JMeq w w' ->
-  field_at sh t gfs v' p |--
-    mapsto sh (nested_field_type t gfs) (field_address t gfs p) v *
-     (mapsto sh (nested_field_type t gfs) (field_address t gfs p) w -*
+  field_at sh t gfs v' p ⊢
+    mapsto sh (nested_field_type t gfs) (field_address t gfs p) v ∗
+     (mapsto sh (nested_field_type t gfs) (field_address t gfs p) w -∗
         field_at sh t gfs w' p).
 Proof.
   intros.
@@ -2379,7 +2314,7 @@ Proof.
   normalize.
   rewrite field_compatible_field_address by auto.
   subst.
-  apply RAMIF_PLAIN.solve with emp; [rewrite sepcon_emp | rewrite emp_sepcon]; auto.
+  iIntros "$ $".
 Qed.
 
 Lemma mapsto_data_at {cs: compspecs} sh t v v' p :  (* not needed here *)
@@ -2390,7 +2325,7 @@ Lemma mapsto_data_at {cs: compspecs} sh t v v' p :  (* not needed here *)
   align_compatible t p ->
   complete_legal_cosu_type t = true ->
   JMeq v v' ->
-  mapsto sh t p v = data_at sh t v' p.
+  mapsto sh t p v ⊣⊢ data_at sh t v' p.
 Proof.
   intros.
   unfold data_at, field_at, at_offset, offset_val.
@@ -2400,7 +2335,7 @@ Proof.
   rewrite by_value_data_at_rec_nonvolatile by auto.
   apply (fun HH => JMeq_trans HH (JMeq_sym (repinject_JMeq _ v' H))) in H5; apply JMeq_eq in H5.
   rewrite prop_true_andp; auto.
-  f_equal. auto.
+  f_equiv; auto.
   repeat split; auto.
 Qed.
 
@@ -2409,7 +2344,7 @@ Lemma mapsto_data_at' {cs: compspecs} sh t v v' p:
   type_is_volatile t = false ->
   field_compatible t nil p ->
   JMeq v v' ->
-  mapsto sh t p v = data_at sh t v' p.
+  mapsto sh t p v ⊣⊢ data_at sh t v' p.
 Proof.
   intros.
   unfold data_at, field_at, at_offset, offset_val.
@@ -2417,7 +2352,7 @@ Proof.
   rewrite prop_true_andp by auto.
   rewrite by_value_data_at_rec_nonvolatile by auto.
   apply (fun HH => JMeq_trans HH (JMeq_sym (repinject_JMeq _ v' H))) in H2; apply JMeq_eq in H2.
-  f_equal; auto.
+  f_equiv; auto.
   destruct H1. destruct p; try contradiction.
   rewrite ptrofs_add_repr_0_r. auto.
 Qed.
@@ -2439,7 +2374,7 @@ Lemma mapsto_data_at'' {cs: compspecs}: forall sh t v v' p,
   ((type_is_by_value t) && (complete_legal_cosu_type t) && (negb (type_is_volatile t)) && is_aligned cenv_cs ha_env_cs la_env_cs t 0 = true)%bool ->
   headptr p ->
   JMeq v v' ->
-  mapsto sh t p v = data_at sh t v' p.
+  mapsto sh t p v ⊣⊢ data_at sh t v' p.
 Proof.
   intros.
   rewrite !andb_true_iff in H.
@@ -2455,34 +2390,31 @@ Qed.
 Lemma data_at_type_changable {cs}: forall (sh: Share.t) (t1 t2: type) v1 v2,
   t1 = t2 ->
   JMeq v1 v2 ->
-  @data_at cs sh t1 v1 = data_at sh t2 v2.
+  data_at (cs := cs) sh t1 v1 = data_at sh t2 v2.
 Proof. intros. subst. apply JMeq_eq in H0. subst v2. reflexivity. Qed.
 
-Lemma field_at_change_composite {cs_from cs_to} {CCE: change_composite_env cs_from cs_to}: forall (sh: Share.t) (t: type) gfs v1 v2,
+Lemma field_at_change_composite {cs_from cs_to} {CCE: change_composite_env cs_from cs_to}: forall (sh: Share.t) (t: type) gfs v1 v2 p,
   JMeq v1 v2 ->
   cs_preserve_type cs_from cs_to (coeq _ _) t = true ->
-  @field_at cs_from sh t gfs v1 = @field_at cs_to sh t gfs v2.
+  field_at (cs := cs_from) sh t gfs v1 p ⊣⊢ field_at (cs := cs_to) sh t gfs v2 p.
 Proof.
   intros.
   unfold field_at.
-  extensionality p.
   apply andp_prop_ext.
   + apply field_compatible_change_composite; auto.
   + intros.
     pose proof H1.
     rewrite field_compatible_change_composite in H2 by auto.
-    f_equal.
-    - revert v1 H;
-      rewrite nested_field_type_change_composite by auto.
-      intros.
-      apply data_at_rec_change_composite; auto.
-      apply nested_field_type_preserves_change_composite; auto.
-    - apply nested_field_offset_change_composite; auto.
+    rewrite nested_field_offset_change_composite by auto.
+    revert v1 H; rewrite nested_field_type_change_composite by auto.
+    intros.
+    apply data_at_rec_change_composite; auto.
+    apply nested_field_type_preserves_change_composite; auto.
 Qed.
 
-Lemma field_at__change_composite {cs_from cs_to} {CCE: change_composite_env cs_from cs_to}: forall (sh: Share.t) (t: type) gfs,
+Lemma field_at__change_composite {cs_from cs_to} {CCE: change_composite_env cs_from cs_to}: forall (sh: Share.t) (t: type) gfs p,
   cs_preserve_type cs_from cs_to (coeq _ _) t = true ->
-  @field_at_ cs_from sh t gfs = @field_at_ cs_to sh t gfs.
+  field_at_ (cs := cs_from) sh t gfs p ⊣⊢ field_at_ (cs := cs_to) sh t gfs p.
 Proof.
   intros.
   apply field_at_change_composite; auto.
@@ -2491,18 +2423,18 @@ Proof.
   apply nested_field_type_preserves_change_composite; auto.
 Qed.
 
-Lemma data_at_change_composite {cs_from cs_to} {CCE: change_composite_env cs_from cs_to}: forall (sh: Share.t) (t: type) v1 v2,
+Lemma data_at_change_composite {cs_from cs_to} {CCE: change_composite_env cs_from cs_to}: forall (sh: Share.t) (t: type) v1 v2 p,
   JMeq v1 v2 ->
   cs_preserve_type cs_from cs_to (coeq _ _) t = true ->
-  @data_at cs_from sh t v1 = @data_at cs_to sh t v2.
+  data_at (cs := cs_from) sh t v1 p ⊣⊢ data_at (cs := cs_to) sh t v2 p.
 Proof.
   intros.
   apply field_at_change_composite; auto.
 Qed.
 
-Lemma data_at__change_composite {cs_from cs_to} {CCE: change_composite_env cs_from cs_to}: forall (sh: Share.t) (t: type),
+Lemma data_at__change_composite {cs_from cs_to} {CCE: change_composite_env cs_from cs_to}: forall (sh: Share.t) (t: type) p,
   cs_preserve_type cs_from cs_to (coeq _ _) t = true ->
-  @data_at_ cs_from sh t = @data_at_ cs_to sh t.
+  data_at_ (cs := cs_from) sh t p ⊣⊢ data_at_ (cs := cs_to) sh t p.
 Proof.
   intros.
   apply field_at__change_composite; auto.
@@ -2513,20 +2445,22 @@ Lemma array_at_data_at1 {cs} : forall sh t gfs lo hi v p,
    lo <= hi ->
    field_compatible0 t (gfs SUB lo) p ->
    field_compatible0 t (gfs SUB hi) p ->
-  @array_at cs sh t gfs lo hi v p =
-  at_offset (@data_at cs sh (nested_field_array_type t gfs lo hi) v)
+  array_at sh t gfs lo hi v p ⊣⊢
+  at_offset (data_at sh (nested_field_array_type t gfs lo hi) v)
                (nested_field_offset t (ArraySubsc lo :: gfs)) p.
 Proof.
-  intros. rewrite array_at_data_at by auto. unfold at_offset. apply pred_ext; normalize.
+  intros. rewrite array_at_data_at by auto. unfold at_offset. apply bi.equiv_entails_2; normalize.
 Qed.
 
-Lemma data_at_ext_derives {cs} sh t v v' p q: v=v' -> p=q -> @data_at cs sh t v p |-- @data_at cs sh t v' q.
+Lemma data_at_ext_derives {cs} sh t v v' p q: v=v' -> p=q -> data_at sh t v p ⊢ data_at sh t v' q.
 Proof. intros; subst.
 apply derives_refl.
 Qed.
 
-Lemma data_at_ext_eq {cs} sh t v v' p q: v=v' -> p=q -> @data_at cs sh t v p = @data_at cs sh t v' q.
+Lemma data_at_ext_eq {cs} sh t v v' p q: v=v' -> p=q -> data_at sh t v p = data_at sh t v' q.
 Proof. intros; subst. trivial. Qed.
+
+End lemmas.
 
 (* does not simplify array indices, because that might be too expensive *)
 Ltac simpl_compute_legal_nested_field :=
@@ -2538,7 +2472,7 @@ Ltac simpl_compute_legal_nested_field :=
 
 Ltac solve_legal_nested_field_in_entailment :=
    match goal with
-   | |- _ |-- !! legal_nested_field ?t_root ?gfs =>
+   | |- _ ⊢ ⌜legal_nested_field ?t_root ?gfs⌝ =>
      try unfold t_root;
      try unfold gfs;
      try match gfs with
@@ -2546,15 +2480,15 @@ Ltac solve_legal_nested_field_in_entailment :=
      end
   end;
   first
-  [ apply prop_right; apply compute_legal_nested_field_spec';
+  [ apply bi.pure_intro; apply compute_legal_nested_field_spec';
     simpl_compute_legal_nested_field;
     repeat apply Forall_cons; try apply Forall_nil; lia
   |
   apply compute_legal_nested_field_spec;
   simpl_compute_legal_nested_field;
   repeat apply Forall_cons; try apply Forall_nil;
-  try solve [apply prop_right; auto; lia];
-  try solve [normalize; apply prop_right; auto; lia]
+  try solve [apply bi.pure_intro; auto; lia];
+  try solve [normalize; apply bi.pure_intro; auto; lia]
   ].
 
 Ltac headptr_field_compatible :=
@@ -2569,25 +2503,22 @@ Ltac headptr_field_compatible :=
 #[export] Hint Extern 2 (field_compatible _ _ _) => headptr_field_compatible : field_compatible.
 
 (* BEGIN New experiments *)
+Section new_lemmas.
+
+Context `{!heapGS Σ}.
 
 Lemma data_at_data_at_cancel  {cs: compspecs}: forall sh t v v' p,
   v = v' ->
-  data_at sh t v p |-- data_at sh t v' p.
+  data_at sh t v p ⊢ data_at sh t v' p.
 Proof. intros. subst. apply derives_refl. Qed.
-
-#[export] Hint Resolve data_at_data_at_cancel : cancel.
-
 
 Lemma field_at_field_at_cancel  {cs: compspecs}: forall sh t gfs v v' p,
   v = v' ->
-  field_at sh t gfs v p |-- field_at sh t gfs v' p.
+  field_at sh t gfs v p ⊢ field_at sh t gfs v' p.
 Proof. intros. subst. apply derives_refl. Qed.
 
-#[export] Hint Resolve data_at_data_at_cancel : cancel.
-#[export] Hint Resolve field_at_field_at_cancel : cancel.
-
 Lemma data_at__data_at {cs: compspecs}:
-   forall sh t v p, v = default_val t -> data_at_ sh t p |-- data_at sh t v p.
+   forall sh t v p, v = default_val t -> data_at_ sh t p ⊢ data_at sh t v p.
 Proof.
 intros; subst; unfold data_at_; apply derives_refl.
 Qed.
@@ -2598,142 +2529,121 @@ Proof.
 Qed.
 
 Lemma data_at_shares_join : forall {cs} sh t v p shs sh1 (Hsplit : sepalg_list.list_join sh1 shs sh),
-  @data_at cs sh1 t v p * iter_sepcon.iter_sepcon (fun sh => data_at sh t v p) shs =
+  data_at sh1 t v p ∗ ([∗ list] sh ∈ shs, data_at sh t v p) ⊣⊢
   data_at sh t v p.
 Proof.
   induction shs; intros; simpl.
   - inv Hsplit.
-    rewrite sepcon_emp; auto.
+    apply bi.sep_emp.
   - inv Hsplit.
-    erewrite <- sepcon_assoc, data_at_share_join; eauto.
+    rewrite assoc, data_at_share_join; eauto; apply _.
 Qed.
 
 Lemma data_at_shares_join_old : forall {cs} sh t v p shs sh1 (Hsplit : sepalg_list.list_join sh1 shs sh),
-  @data_at cs sh1 t v p * fold_right sepcon emp (map (fun sh => data_at sh t v p) shs) =
+  data_at sh1 t v p ∗ fold_right bi_sep emp (map (fun sh => data_at sh t v p) shs) ⊣⊢
   data_at sh t v p.
 Proof.
   induction shs; intros; simpl.
   - inv Hsplit.
-    rewrite sepcon_emp; auto.
+    apply bi.sep_emp.
   - inv Hsplit.
-    erewrite <- sepcon_assoc, data_at_share_join; eauto.
+    rewrite assoc, data_at_share_join; eauto; apply _.
 Qed.
 
 Lemma struct_pred_value_cohere : forall {cs : compspecs} m sh1 sh2 p t f off v1 v2
   (Hsh1 : readable_share sh1) (Hsh2 : readable_share sh2)
   (IH : Forall (fun it : member => forall v1 v2 (p : val),
         readable_share sh1 -> readable_share sh2 ->
-        data_at_rec sh1 (t it) v1 p * data_at_rec sh2 (t it) v2 p |--
-        data_at_rec sh1 (t it) v1 p * data_at_rec sh2 (t it) v1 p) m),
+        data_at_rec sh1 (t it) v1 p ∗ data_at_rec sh2 (t it) v2 p ⊢
+        data_at_rec sh1 (t it) v1 p ∗ data_at_rec sh2 (t it) v1 p) m),
   struct_pred m (fun (it : member) v =>
-    withspacer sh1 (f it + sizeof (t it)) (off it) (at_offset (data_at_rec sh1 (t it) v) (f it))) v1 p *
+    withspacer sh1 (f it + sizeof (t it)) (off it) (at_offset (data_at_rec sh1 (t it) v) (f it))) v1 p ∗
   struct_pred m (fun (it : member) v =>
-    withspacer sh2 (f it + sizeof (t it)) (off it) (at_offset (data_at_rec sh2 (t it) v) (f it))) v2 p |--
+    withspacer sh2 (f it + sizeof (t it)) (off it) (at_offset (data_at_rec sh2 (t it) v) (f it))) v2 p ⊢
   struct_pred m (fun (it : member) v =>
-    withspacer sh1 (f it + sizeof (t it)) (off it) (at_offset (data_at_rec sh1 (t it) v) (f it))) v1 p *
+    withspacer sh1 (f it + sizeof (t it)) (off it) (at_offset (data_at_rec sh1 (t it) v) (f it))) v1 p ∗
   struct_pred m (fun (it : member) v =>
     withspacer sh2 (f it + sizeof (t it)) (off it) (at_offset (data_at_rec sh2 (t it) v) (f it))) v1 p.
 Proof.
   intros.
   revert v1 v2; induction m; auto; intros.
-  apply derives_refl.
   inv IH.
   destruct m.
   - unfold withspacer, at_offset; simpl.
     if_tac; auto.
-    match goal with |- (?P1 * ?Q1) * (?P2 * ?Q2) |-- _ => apply derives_trans with (Q := (P1 * P2) * (Q1 * Q2));
+    match goal with |- (?P1 ∗ ?Q1) ∗ (?P2 ∗ ?Q2) ⊢ _ => trans ((P1 ∗ P2) ∗ (Q1 ∗ Q2));
       [cancel|] end.
-    eapply derives_trans; [apply sepcon_derives, derives_refl|].
-    { apply H1; auto. }
+    rewrite H1; auto.
     cancel.
   - rewrite !struct_pred_cons2.
-    match goal with |- (?P1 * ?Q1) * (?P2 * ?Q2) |-- _ => apply derives_trans with (Q := (P1 * P2) * (Q1 * Q2));
+    match goal with |- (?P1 ∗ ?Q1) ∗ (?P2 ∗ ?Q2) ⊢ _ => trans ((P1 ∗ P2) ∗ (Q1 ∗ Q2));
       [cancel|] end.
-    match goal with |- _ |-- (?P1 * ?Q1) * (?P2 * ?Q2) => apply derives_trans with (Q := (P1 * P2) * (Q1 * Q2));
+    match goal with |- _ ⊢ (?P1 ∗ ?Q1) ∗ (?P2 ∗ ?Q2) => trans ((P1 ∗ P2) ∗ (Q1 ∗ Q2));
       [|cancel] end.
-    apply sepcon_derives; [|auto].
+    apply bi.sep_mono; auto.
     unfold withspacer, at_offset; simpl.
     if_tac; auto.
-    match goal with |- (?P1 * ?Q1) * (?P2 * ?Q2) |-- _ => apply derives_trans with (Q := (P1 * P2) * (Q1 * Q2));
+    match goal with |- (?P1 ∗ ?Q1) ∗ (?P2 ∗ ?Q2) ⊢ _ => trans ((P1 ∗ P2) ∗ (Q1 ∗ Q2));
       [cancel|] end.
-    eapply derives_trans; [apply sepcon_derives, derives_refl|].
-    { apply H1; auto. }
+    rewrite H1; auto.
     cancel.
 Qed.
 
 Lemma mapsto_value_eq: forall sh1 sh2 t p v1 v2, readable_share sh1 -> readable_share sh2 ->
-  v1 <> Vundef -> v2 <> Vundef -> mapsto sh1 t p v1 * mapsto sh2 t p v2 |-- !!(v1 = v2).
+  v1 <> Vundef -> v2 <> Vundef -> mapsto sh1 t p v1 ∗ mapsto sh2 t p v2 ⊢ ⌜v1 = v2⌝.
 Proof.
   intros; unfold mapsto.
-  destruct (access_mode t); try solve [rewrite FF_sepcon; apply FF_left].
-  destruct (type_is_volatile t); try solve [rewrite FF_sepcon; apply FF_left].
-  destruct p; try solve [rewrite FF_sepcon; apply FF_left].
-  destruct (readable_share_dec sh1); [|contradiction n; auto].
-  destruct (readable_share_dec sh2); [|contradiction n; auto].
-
-  Transparent mpred.
-  rewrite !prop_false_andp with (P := v1 = Vundef), !orp_FF; auto; Intros.
-  rewrite !prop_false_andp with (P := v2 = Vundef), !orp_FF; auto; Intros.
-  Opaque mpred.
-  constructor; apply res_predicates.address_mapsto_value_cohere.
+  destruct (access_mode t); try solve [iIntros "([] & _)"].
+  destruct (type_is_volatile t); try solve [iIntros "([] & _)"].
+  destruct p; try solve [iIntros "([] & _)"].
+  rewrite !if_true by done.
+  iIntros "([(_ & H1) | (-> & % & H1)] & [(_ & H2) | (-> & % & H2)])"; try solve [exfalso; pose proof (JMeq_refl Vundef); done];
+    iApply res_predicates.address_mapsto_value_cohere; iFrame.
 Qed.
 
 Lemma mapsto_value_cohere: forall sh1 sh2 t p v1 v2, readable_share sh1 ->
-  mapsto sh1 t p v1 * mapsto sh2 t p v2 |-- mapsto sh1 t p v1 * mapsto sh2 t p v1.
+  mapsto sh1 t p v1 ∗ mapsto sh2 t p v2 ⊢ mapsto sh1 t p v1 ∗ mapsto sh2 t p v1.
 Proof.
   intros; unfold mapsto.
   destruct (access_mode t); try simple apply derives_refl.
   destruct (type_is_volatile t); try simple apply derives_refl.
   destruct p; try simple apply derives_refl.
-  destruct (readable_share_dec sh1); [|contradiction n; auto].
+  rewrite if_true by done.
   destruct (eq_dec v1 Vundef).
-  Transparent mpred.
-  - subst; rewrite !prop_false_andp with (P := tc_val t Vundef), !FF_orp, prop_true_andp; auto;
+  - subst; rewrite !prop_false_andp with (P := tc_val t Vundef), !bi.False_or, prop_true_andp; auto;
       try apply tc_val_Vundef.
     cancel.
-    rewrite prop_true_andp with (P := Vundef = Vundef); auto.
     if_tac.
-    + apply orp_left; Intros; auto.
-      Exists v2; auto.
-    + Intros. apply andp_right; auto. apply prop_right; split; auto. hnf; intros. contradiction H3; auto.
-  - rewrite !prop_false_andp with (P := v1 = Vundef), !orp_FF; auto; Intros.
-    apply andp_right; [apply prop_right; auto|].
+    + iIntros "[(% & ?) | (% & ?)]"; iRight; auto.
+    + Intros. iIntros "$"; iPureIntro; repeat split; auto. apply tc_val'_Vundef.
+  - rewrite !prop_false_andp with (P := v1 = Vundef), !bi.or_False; auto; Intros.
+    apply bi.and_intro; [apply bi.pure_intro; auto|].
     if_tac.
-    eapply derives_trans with (Q := _ * EX v2' : val,
-      res_predicates.address_mapsto m v2' _ _);
-      [apply sepcon_derives; [apply derives_refl|]|].
-    + destruct (eq_dec v2 Vundef).
-      * subst; rewrite prop_false_andp with (P := tc_val t Vundef), FF_orp;
-          try apply tc_val_Vundef.
-        rewrite prop_true_andp with (P := Vundef = Vundef); auto.  apply derives_refl.
-      * rewrite prop_false_andp with (P := v2 = Vundef), orp_FF; auto; Intros.
-        Exists v2; auto.
-    + Intro v2'.
-      assert_PROP (v1 = v2') by (constructor; apply res_predicates.address_mapsto_value_cohere).
-      subst. apply sepcon_derives; auto. apply andp_right; auto.
-      apply prop_right; auto.
-    + apply sepcon_derives; auto.
-      Intros. apply andp_right; auto.
-      apply prop_right; split; auto.
-      intro; auto.
-Opaque mpred.
+    + iIntros "(H1 & H2)".
+      iAssert (∃ v2' : val, res_predicates.address_mapsto m v2' _ _) with "[H2]" as (v2') "H2".
+      { iDestruct "H2" as "[(% & ?) | (_ & $)]"; auto. }
+      iAssert ⌜v1 = v2'⌝ as %->. { iApply res_predicates.address_mapsto_value_cohere; iFrame. }
+      iFrame; eauto.
+    + apply bi.sep_mono; first done.
+      iIntros "((% & %) & $)"; iPureIntro; repeat split; auto.
+      apply tc_val_tc_val'; auto.
 Qed.
 
 Lemma data_at_value_cohere : forall {cs : compspecs} sh1 sh2 t v1 v2 p, readable_share sh1 ->
   type_is_by_value t = true -> type_is_volatile t = false ->
-  data_at sh1 t v1 p * data_at sh2 t v2 p |--
-  data_at sh1 t v1 p * data_at sh2 t v1 p.
+  data_at sh1 t v1 p ∗ data_at sh2 t v2 p ⊢
+  data_at sh1 t v1 p ∗ data_at sh2 t v1 p.
 Proof.
-  intros; unfold data_at, field_at, at_offset; Intros.
-  apply andp_right; [apply prop_right; auto|].
+  intros; unfold data_at, field_at, at_offset.
+  iIntros "((% & ?) & (% & ?))".
   rewrite !by_value_data_at_rec_nonvolatile by auto.
-  apply mapsto_value_cohere; auto.
+  iDestruct (mapsto_value_cohere with "[-]") as "($ & $)"; auto; iFrame.
 Qed.
 
 Lemma data_at_value_eq : forall {cs : compspecs} sh1 sh2 t v1 v2 p,
   readable_share sh1 -> readable_share sh2 ->
   is_pointer_or_null v1 -> is_pointer_or_null v2 ->
-  data_at sh1 (tptr t) v1 p * data_at sh2 (tptr t) v2 p |-- !! (v1 = v2).
+  data_at sh1 (tptr t) v1 p ∗ data_at sh2 (tptr t) v2 p ⊢ ⌜v1 = v2⌝.
 Proof.
   intros; unfold data_at, field_at, at_offset; Intros.
   rewrite !by_value_data_at_rec_nonvolatile by auto.
@@ -2744,60 +2654,69 @@ Qed.
 
 Lemma data_at_array_value_cohere : forall {cs : compspecs} sh1 sh2 t z a v1 v2 p, readable_share sh1 ->
   type_is_by_value t = true -> type_is_volatile t = false ->
-  data_at sh1 (Tarray t z a) v1 p * data_at sh2 (Tarray t z a) v2 p |--
-  data_at sh1 (Tarray t z a) v1 p * data_at sh2 (Tarray t z a) v1 p.
+  data_at sh1 (Tarray t z a) v1 p ∗ data_at sh2 (Tarray t z a) v2 p ⊢
+  data_at sh1 (Tarray t z a) v1 p ∗ data_at sh2 (Tarray t z a) v1 p.
 Proof.
-  intros; unfold data_at, field_at, at_offset; Intros.
-  apply andp_right; [apply prop_right; auto|].
+  intros; unfold data_at, field_at, at_offset.
+  iIntros "((% & H1) & (_ & H2))".
+  rewrite !bi.pure_True, !bi.True_and by done.
   rewrite !data_at_rec_eq; simpl.
-  unfold array_pred, aggregate_pred.array_pred. Intros.
-  apply andp_right; [apply prop_right; auto|].
+  unfold array_pred, aggregate_pred.array_pred.
+  iDestruct "H1" as (?) "H1"; iDestruct "H2" as (?) "H2".
+  rewrite !bi.pure_True, !bi.True_and by done.
   rewrite Z.sub_0_r in *.
-  erewrite aggregate_pred.rangespec_ext by (intros; rewrite Z.sub_0_r; apply f_equal; auto).
-  setoid_rewrite aggregate_pred.rangespec_ext at 2; [|intros; rewrite Z.sub_0_r; apply f_equal; auto].
-  setoid_rewrite aggregate_pred.rangespec_ext at 4; [|intros; rewrite Z.sub_0_r; apply f_equal; auto].
-  clear H3 H4.
   rewrite Z2Nat_max0 in *.
-  forget (offset_val 0 p) as p'; forget (Z.to_nat z) as n; forget 0 as lo; revert dependent lo; induction n; auto; simpl; intros.
- apply derives_refl.
-  match goal with |- (?P1 * ?Q1) * (?P2 * ?Q2) |-- _ =>
-    eapply derives_trans with (Q := (P1 * P2) * (Q1 * Q2)); [cancel|] end.
-  eapply derives_trans; [apply sepcon_derives|].
-  - unfold at_offset.
-    rewrite 2by_value_data_at_rec_nonvolatile by auto.
-    apply mapsto_value_cohere; auto.
-  - apply IHn.
-  - unfold at_offset; rewrite 2by_value_data_at_rec_nonvolatile by auto; cancel.
+  clear H3 H4.
+  forget (offset_val 0 p) as p'; forget (Z.to_nat z) as n.
+  set (lo := 0) at 1 3 5 7; clearbody lo.
+  iInduction n as [|] "IH" forall (lo); auto; simpl; intros.
+  iDestruct "H1" as "(H1a & H1b)"; iDestruct "H2" as "(H2a & H2b)".
+  unfold at_offset.
+  rewrite !by_value_data_at_rec_nonvolatile by auto.
+  iDestruct (mapsto_value_cohere with "[$H1a $H2a]") as "($ & $)".
+  iApply ("IH" with "H1b H2b").
 Qed.
 
 Lemma field_at_array_inbounds : forall {cs : compspecs} sh t z a i v p,
-  field_at sh (Tarray t z a) (ArraySubsc i :: nil) v p |-- !!(0 <= i < z).
+  field_at sh (Tarray t z a) (ArraySubsc i :: nil) v p ⊢ ⌜0 <= i < z⌝.
 Proof.
   intros. rewrite field_at_compatible'.
-  apply derives_extract_prop. intros.
-  apply prop_right.
+  apply bi.pure_elim_l. intros.
+  apply bi.pure_intro.
   destruct H as (_ & _ & _ & _ & _ & ?); auto.
 Qed.
 
 Lemma field_at__field_at {cs: compspecs} :
-   forall sh t gfs v p, v = default_val (nested_field_type t gfs) -> field_at_ sh t gfs p |-- field_at sh t gfs v p.
+   forall sh t gfs v p, v = default_val (nested_field_type t gfs) -> field_at_ sh t gfs p ⊢ field_at sh t gfs v p.
 Proof.
 intros; subst; unfold field_at_; apply derives_refl.
 Qed.
 
 Lemma data_at__field_at {cs: compspecs}:
-   forall sh t v p, v = default_val t -> data_at_ sh t p |-- field_at sh t nil v p.
+   forall sh t v p, v = default_val t -> data_at_ sh t p ⊢ field_at sh t nil v p.
 Proof.
 intros; subst; unfold data_at_; apply derives_refl.
 Qed.
 
 Lemma field_at__data_at {cs: compspecs} :
-   forall sh t v p, v = default_val (nested_field_type t nil) -> field_at_ sh t nil p |-- data_at sh t v p.
+   forall sh t v p, v = default_val (nested_field_type t nil) -> field_at_ sh t nil p ⊢ data_at sh t v p.
 Proof.
 intros; subst; unfold field_at_; apply derives_refl.
 Qed.
 
+Lemma field_at_data_at_cancel': forall {cs : compspecs} sh t v p,
+  field_at sh t nil v p ⊣⊢ data_at sh t v p.
+Proof.
+  intros. apply bi.equiv_entails_2.
+  apply field_at_data_at_cancel.
+  apply data_at_field_at_cancel.
+Qed.
 
+End new_lemmas.
+
+#[export] Hint Resolve data_at_data_at_cancel : cancel.
+#[export] Hint Resolve data_at_data_at_cancel : cancel.
+#[export] Hint Resolve field_at_field_at_cancel : cancel.
 #[export] Hint Resolve data_at__data_at : cancel.
 #[export] Hint Resolve field_at__field_at : cancel.
 #[export] Hint Resolve data_at__field_at : cancel.
@@ -2814,14 +2733,6 @@ Qed.
 
 (* enhance cancel to solve field_at and data_at *)
 
-Lemma field_at_data_at_cancel': forall {cs : compspecs} sh t v p,
-  field_at sh t nil v p = data_at sh t v p.
-Proof.
-  intros. apply pred_ext.
-  apply field_at_data_at_cancel.
-  apply data_at_field_at_cancel.
-Qed.
-
 #[export] Hint Rewrite
   @field_at_data_at_cancel'
   @field_at_data_at
@@ -2830,18 +2741,15 @@ Qed.
 
 (* END new experiments *)
 
+Section more_lemmas.
+
+Context `{!heapGS Σ}.
 
 Lemma data_at__Tarray:
   forall {CS: compspecs} sh t n a,
   data_at_ sh (Tarray t n a) =
   data_at sh (Tarray t n a) (Zrepeat (default_val t) n).
-Proof.
-intros.
-unfold data_at_, field_at_, data_at.
-extensionality p.
-simpl.
-f_equal.
-Qed.
+Proof. reflexivity. Qed.
 
 Lemma data_at__tarray:
   forall {CS: compspecs} sh t n,
@@ -2854,13 +2762,7 @@ Lemma data_at__Tarray':
   v = Zrepeat (default_val t) n ->
   data_at_ sh (Tarray t n a) = data_at sh (Tarray t n a) v.
 Proof.
-intros.
-unfold data_at_, field_at_, data_at.
-extensionality p.
-simpl.
-f_equal.
-subst.
-reflexivity.
+intros. subst; reflexivity.
 Qed.
 
 Lemma data_at__tarray':
@@ -2868,26 +2770,6 @@ Lemma data_at__tarray':
   v = Zrepeat (default_val t) n ->
   data_at_ sh (tarray t n) = data_at sh (tarray t n) v.
 Proof. intros; apply data_at__Tarray'; auto. Qed.
-
-Ltac unfold_data_at_ p :=
- match goal with |- context [data_at_ ?sh ?t p] =>
-  let d := fresh "d" in set (d := data_at_ sh t p);
-  pattern d;
-  let g := fresh "goal" in
-   match goal with |- ?G d => set (g:=G) end;
-  revert d;
-  match t with
-   | Tarray ?t1 ?n _ =>
-          erewrite data_at__Tarray' by apply eq_refl;
-          try change (default_val t1) with Vundef
-   | tarray ?t1 ?n =>
-          erewrite data_at__tarray' by apply eq_refl;
-          try change (default_val t1) with Vundef
-   | _ => change (data_at_ sh t p) with (data_at sh t (default_val t) p);
-              try change (default_val t) with Vundef
-  end;
-  subst g; intro d; subst d; cbv beta
- end.
 
 Lemma change_compspecs_field_at_cancel:
   forall {cs1 cs2: compspecs} {CCE : change_composite_env cs1 cs2}
@@ -2898,13 +2780,11 @@ Lemma change_compspecs_field_at_cancel:
     t1 = t2 ->
     cs_preserve_type cs1 cs2 (@coeq cs1 cs2 CCE) t1 = true ->
    JMeq v1 v2 ->
-   @field_at cs1 sh t1 gfs v1 p |-- @field_at cs2 sh t2 gfs v2 p.
+   field_at (cs := cs1) sh t1 gfs v1 p ⊢ field_at (cs := cs2) sh t2 gfs v2 p.
 Proof.
 intros.
 subst t2.
-apply derives_refl'.
-apply equal_f.
-apply @field_at_change_composite with CCE; auto.
+rewrite @field_at_change_composite with CCE; auto.
 Qed.
 
 Lemma change_compspecs_data_at_cancel:
@@ -2915,7 +2795,7 @@ Lemma change_compspecs_data_at_cancel:
     t1 = t2 ->
     cs_preserve_type cs1 cs2 (@coeq cs1 cs2 CCE) t1 = true ->
    JMeq v1 v2 ->
-   @data_at cs1 sh t1 v1 p |-- @data_at cs2 sh t2 v2 p.
+   data_at (cs := cs1) sh t1 v1 p ⊢ data_at (cs := cs2) sh t2 v2 p.
 Proof.
 intros.
 apply change_compspecs_field_at_cancel; auto.
@@ -2927,7 +2807,7 @@ Lemma change_compspecs_field_at_cancel2:
         (p: val),
     t1 = t2 ->
     cs_preserve_type cs1 cs2 (@coeq cs1 cs2 CCE) t1 = true ->
-   @field_at_ cs1 sh t1 gfs p |-- @field_at_ cs2 sh t2 gfs p.
+   field_at_ (cs := cs1) sh t1 gfs p ⊢ field_at_ (cs := cs2) sh t2 gfs p.
 Proof.
 intros.
 subst t2.
@@ -2944,7 +2824,7 @@ Lemma change_compspecs_data_at_cancel2:
         (p: val),
     t1 = t2 ->
     cs_preserve_type cs1 cs2 (@coeq cs1 cs2 CCE) t1 = true ->
-   @data_at_ cs1 sh t1 p |-- @data_at_ cs2 sh t2 p.
+   data_at_ (cs := cs1) sh t1 p ⊢ data_at_ (cs := cs2) sh t2 p.
 Proof.
 intros.
 apply change_compspecs_field_at_cancel2; auto.
@@ -2957,12 +2837,11 @@ Lemma change_compspecs_field_at_cancel3:
         (p: val),
     t1 = t2 ->
     cs_preserve_type cs1 cs2 (@coeq cs1 cs2 CCE) t1 = true ->
-   @field_at cs1 sh t1 gfs v1 p |-- @field_at_ cs2 sh t2 gfs p.
+   field_at (cs := cs1) sh t1 gfs v1 p ⊢ field_at_ (cs := cs2) sh t2 gfs p.
 Proof.
 intros.
 subst t2.
-apply derives_trans with (@field_at_ cs1 sh t1 gfs p).
-apply field_at_field_at_.
+rewrite field_at_field_at_.
 apply @change_compspecs_field_at_cancel2 with CCE; auto.
 Qed.
 
@@ -2973,65 +2852,32 @@ Lemma change_compspecs_data_at_cancel3:
         (p: val),
     t1 = t2 ->
     cs_preserve_type cs1 cs2 (@coeq cs1 cs2 CCE) t1 = true ->
-   @data_at cs1 sh t1 v1 p |-- @data_at_ cs2 sh t2 p.
+   data_at (cs := cs1) sh t1 v1 p ⊢ data_at_ (cs := cs2) sh t2 p.
 Proof.
 intros.
 apply @change_compspecs_field_at_cancel3 with CCE; auto.
 Qed.
 
-#[export] Hint Extern 2 (@data_at_ ?cs1 ?sh _ ?p |-- @data_at_ ?cs2 ?sh _ ?p) =>
-    (tryif constr_eq cs1 cs2 then fail
-     else simple apply change_compspecs_data_at_cancel2; reflexivity) : cancel.
-
-#[export] Hint Extern 2 (@data_at ?cs1 ?sh _ _ ?p |-- @data_at_ ?cs2 ?sh _ ?p) =>
-    (tryif constr_eq cs1 cs2 then fail
-     else simple apply change_compspecs_data_at_cancel3; reflexivity) : cancel.
-
-#[export] Hint Extern 2 (@data_at ?cs1 ?sh _ _ ?p |-- @data_at ?cs2 ?sh _ _ ?p) =>
-    (tryif constr_eq cs1 cs2 then fail
-     else simple apply change_compspecs_data_at_cancel;
-       [ reflexivity | reflexivity | apply JMeq_refl]) : cancel.
-
-#[export] Hint Extern 2 (@field_at_ ?cs1 ?sh _ ?gfs ?p |-- @field_at_ ?cs2 ?sh _ ?gfs ?p) =>
-    (tryif constr_eq cs1 cs2 then fail
-     else simple apply change_compspecs_field_at_cancel2; reflexivity) : cancel.
-
-#[export] Hint Extern 2 (@field_at ?cs1 ?sh _ ?gfs _ ?p |-- @field_at_ ?cs2 ?sh _ ?gfs ?p) =>
-    (tryif constr_eq cs1 cs2 then fail
-     else simple apply change_compspecs_field_at_cancel3; reflexivity) : cancel.
-
-#[export] Hint Extern 2 (@field_at ?cs1 ?sh _ ?gfs _ ?p |-- @field_at ?cs2 ?sh _ ?gfs _ ?p) =>
-    (tryif constr_eq cs1 cs2 then fail
-     else simple apply change_compspecs_field_at_cancel;
-        [ reflexivity | reflexivity | apply JMeq_refl]) : cancel.
-
 Lemma data_at_nullptr:
  forall {cs: compspecs} sh t p,
-  data_at sh size_t nullval p =
+  data_at sh size_t nullval p ⊣⊢
   data_at sh (tptr t) nullval p.
 Proof.
 intros.
 unfold data_at, field_at.
-f_equal.
-f_equal.
+apply bi.and_proper.
+f_equiv.
 unfold field_compatible; simpl.
-f_equal; auto.
-f_equal; auto.
-f_equal.
-f_equal.
-unfold align_compatible.
-destruct p; try auto.
-apply prop_ext; split; intro;
-(eapply align_compatible_rec_by_value_inv in H; [ | reflexivity];
+intuition; destruct p; try auto;
+(eapply align_compatible_rec_by_value_inv in H2; [ | reflexivity];
  eapply align_compatible_rec_by_value; [reflexivity | ];
- apply H).
-simpl.
+ apply H2).
 unfold at_offset.
 rewrite !by_value_data_at_rec_nonvolatile by reflexivity.
 simpl.
 unfold nested_field_type; simpl.
-rewrite <- mapsto_size_t_tptr_nullval with (t:=t).
-f_equal.
+rewrite <- mapsto_tuint_tptr_nullval with (t:=t).
+done.
 Qed.
 
 Lemma data_at_int_or_ptr_int:
@@ -3054,8 +2900,6 @@ Proof.
   eapply align_compatible_rec_by_value_inv in H;
    try reflexivity;
   try (eapply align_compatible_rec_by_value; eauto).
-  reflexivity.
-  reflexivity.
 Qed.
 
 Lemma data_at_int_or_ptr_ptr:
@@ -3081,8 +2925,6 @@ Proof.
   eapply align_compatible_rec_by_value_inv in H;
    try reflexivity;
   try (eapply align_compatible_rec_by_value; eauto).
-  reflexivity.
-  reflexivity.
  unfold at_offset.
  unfold nested_field_type;  simpl.
  unfold data_at_rec; simpl.
@@ -3102,3 +2944,51 @@ Proof.
  rewrite N.eqb_refl.
  rewrite andb_false_r. reflexivity.
 Qed.
+
+End more_lemmas.
+
+Ltac unfold_data_at_ p :=
+ match goal with |- context [data_at_ ?sh ?t p] =>
+  let d := fresh "d" in set (d := data_at_ sh t p);
+  pattern d;
+  let g := fresh "goal" in
+   match goal with |- ?G d => set (g:=G) end;
+  revert d;
+  match t with
+   | Tarray ?t1 ?n _ =>
+          erewrite data_at__Tarray' by apply eq_refl;
+          try change (default_val t1) with Vundef
+   | tarray ?t1 ?n =>
+          erewrite data_at__tarray' by apply eq_refl;
+          try change (default_val t1) with Vundef
+   | _ => change (data_at_ sh t p) with (data_at sh t (default_val t) p);
+              try change (default_val t) with Vundef
+  end;
+  subst g; intro d; subst d; cbv beta
+ end.
+
+#[export] Hint Extern 2 (@data_at_ ?cs1 ?sh _ ?p ⊢ @data_at_ ?cs2 ?sh _ ?p) =>
+    (tryif constr_eq cs1 cs2 then fail
+     else simple apply change_compspecs_data_at_cancel2; reflexivity) : cancel.
+
+#[export] Hint Extern 2 (@data_at ?cs1 ?sh _ _ ?p ⊢ @data_at_ ?cs2 ?sh _ ?p) =>
+    (tryif constr_eq cs1 cs2 then fail
+     else simple apply change_compspecs_data_at_cancel3; reflexivity) : cancel.
+
+#[export] Hint Extern 2 (@data_at ?cs1 ?sh _ _ ?p ⊢ @data_at ?cs2 ?sh _ _ ?p) =>
+    (tryif constr_eq cs1 cs2 then fail
+     else simple apply change_compspecs_data_at_cancel;
+       [ reflexivity | reflexivity | apply JMeq_refl]) : cancel.
+
+#[export] Hint Extern 2 (@field_at_ ?cs1 ?sh _ ?gfs ?p ⊢ @field_at_ ?cs2 ?sh _ ?gfs ?p) =>
+    (tryif constr_eq cs1 cs2 then fail
+     else simple apply change_compspecs_field_at_cancel2; reflexivity) : cancel.
+
+#[export] Hint Extern 2 (@field_at ?cs1 ?sh _ ?gfs _ ?p ⊢ @field_at_ ?cs2 ?sh _ ?gfs ?p) =>
+    (tryif constr_eq cs1 cs2 then fail
+     else simple apply change_compspecs_field_at_cancel3; reflexivity) : cancel.
+
+#[export] Hint Extern 2 (@field_at ?cs1 ?sh _ ?gfs _ ?p ⊢ @field_at ?cs2 ?sh _ ?gfs _ ?p) =>
+    (tryif constr_eq cs1 cs2 then fail
+     else simple apply change_compspecs_field_at_cancel;
+        [ reflexivity | reflexivity | apply JMeq_refl]) : cancel.
